makes branch one-shot by removing all multi-shot stuff

theories/case_studies/asynchronous.v
@@ -67,7 +67,7 @@ Definition runner : val :=
 
     let: "fulfill" := 
       (rec: "fulfill" <> := λ: "promise" "comp",   
-        deep-try-os: "comp" #() with
+        deep-try: "comp" #() with
           effect (λ: "x" "k", 
             match: "x" with 
               InjL "x" => 
@@ -113,41 +113,41 @@ Section typing.
 
   Definition Promise τ := Refᶜ (Status τ).
 
-  Definition asig := ⟨μ∀TS: θ, α, ( () -{ ⟨θ,⟩ }-∘ '! α ) + Promise ('! α) ⇒ 
-                                     Promise ('! α)       + '! α, @sem_sig_nil Σ⟩%R. 
+  Definition asig : sem_sig Σ := (μ∀TS: θ, α, ( () -{ θ }-∘ '! α ) + Promise ('! α) ⇒ 
+                                              Promise ('! α)       + '! α)%S. 
 
-  Definition iter_ty τ := (∀R: θ, (τ -{ ⟨θ.1,⟩ }-> ()) → List τ -{ ⟨θ.1,⟩ }-∘ ())%T.
+  Definition iter_ty τ := (∀S: θ, (τ -{ θ }-> ()) → List τ -{ θ }-∘ ())%T.
   
   Definition next_ty := (() → ())%T.
 
   Definition add_ty := ((() ⊸ ()) → ())%T.
 
-  Definition resume_task_ty := (∀T: α,, '! α → ('! α ⊸ ()) → ())%T.
+  Definition resume_task_ty := (∀T: α, '! α → ('! α ⊸ ()) → ())%T.
   
-  Definition runner_ty := (∀T: α,, (() -{ asig }-∘ '! α) → '! α)%T.
+  Definition runner_ty := (∀T: α, (() -{ asig }-∘ '! α) → '! α)%T.
 
   Lemma impossible_typed τ :
-    ⊢ ⊨ impossible : ⟨⟩ : τ.
+    ⊢ ⊨ impossible : ⊥ : τ.
   Proof.
     iIntros. rewrite /impossible.
-    iApply sem_typed_app; first solve_copy; last (iApply sem_typed_unit).
+    iApply sem_typed_app; last (iApply sem_typed_unit).
     rewrite - {1} (app_nil_r []).
     iApply sem_typed_sub_ty; [iApply ty_le_u2aarr|].
     iApply sem_typed_ufun; solve_sidecond. simpl.
-    iApply sem_typed_app; first solve_copy; last (iApply sem_typed_unit).
+    iApply sem_typed_app; last (iApply sem_typed_unit).
     iApply sem_typed_sub_ty; [iApply ty_le_u2aarr|].
     iApply sem_typed_var.
   Qed.
 
   Lemma async_typed :
-    ⊢ ⊨ᵥ async : (∀T: α ,, (() -{ asig }-∘ '! α) -{ asig }-> Promise ('! α)).
+    ⊢ ⊨ᵥ async : (∀T: α , (() -{ asig }-∘ '! α) -{ asig }-> Promise ('! α)).
   Proof.
     rewrite /async. iIntros.
     iApply sem_typed_Tclosure. iIntros (α).
     rewrite - {1} (app_nil_r []).
     iApply sem_typed_ufun; solve_sidecond. simpl.
     iApply (sem_typed_match _ []); solve_sidecond.
-    - iApply (sem_typed_perform_os with "[]");
+    - iApply (sem_typed_perform with "[]");
         try (rewrite /Promise /Status; intros ???????; by repeat f_equiv).
         iApply sem_typed_left_inj.
         iApply sem_typed_sub_nil.
@@ -158,17 +158,17 @@ Section typing.
   Qed.
 
   Lemma await_typed :
-    ⊢ ⊨ᵥ await : (∀T: α ,, Promise ('! α) -{ asig }-> '! α).
+    ⊢ ⊨ᵥ await : (∀T: α, Promise ('! α) -{ asig }-> '! α).
   Proof.
     rewrite /await. iIntros.
     iApply sem_typed_Tclosure. iIntros (α).
     rewrite - {1} (app_nil_r []).
     iApply sem_typed_ufun; solve_sidecond. simpl.
     iApply (sem_typed_match _ [("f", _)]); solve_sidecond.
-    - iApply (sem_typed_perform_os with "[]");
+    - iApply (sem_typed_perform with "[]");
       try (rewrite /Promise /Status; intros ???????; by repeat f_equiv).
       iApply sem_typed_sub_nil. iApply sem_typed_right_inj. iApply sem_typed_var. 
-    - simpl. iApply sem_typed_app_os.
+    - simpl. iApply sem_typed_app.
       { iApply sem_typed_sub_nil. 
         iApply sem_typed_sub_ty; [iApply ty_le_u2aarr|iApply sem_typed_var]. }
       iApply sem_typed_sub_nil. iApply sem_typed_var.
@@ -181,15 +181,15 @@ Section typing.
     ⊢ ⊨ᵥ yield : ( () -{ asig }-> () ).
   Proof.
     iIntros. iApply sem_typed_closure; try done. simpl.
-    iApply (sem_typed_app_os _ [] _ _ _ (Promise ('! ()))).
+    iApply (sem_typed_app _ [] _ _ _ (Promise ('! ()))).
     - iApply sem_typed_sub_ty; [iApply ty_le_u2aarr|].
       iApply sem_typed_sub_ty; [iApply ty_le_uarr|]; 
-        [iApply sigs_le_refl|iApply ty_le_refl|iApply ty_le_cpy_inv|].
+        [iApply sig_le_refl|iApply ty_le_refl|iApply ty_le_cpy_inv|].
       iApply sem_typed_sub_nil. simpl. rewrite -/asig.
       set C := (λ α, (Promise ('! α)) -{ asig }-> ('! α)).
       rewrite -/(C ()). iApply sem_typed_TApp; first solve_copy.
       iApply sem_typed_val. iApply await_typed.
-    - iApply (sem_typed_app _ [] _ _ _ (() -{ asig }-∘ '! ())); first solve_copy.
+    - iApply (sem_typed_app _ [] _ _ _ (() -{ asig }-∘ '! ())).
       + iApply sem_typed_sub_nil. 
         iApply sem_typed_sub_ty; [iApply ty_le_u2aarr|].
         set C := (λ α, (() -{ asig }-∘ '! α) -{ asig }-> Promise ('! α)).
@@ -206,14 +206,14 @@ Section typing.
   Lemma iter_typed τ :
     ⊢ ⊨ᵥ iter : iter_ty τ.
   Proof.
-    iApply sem_typed_Rclosure. iIntros (ρ).
+    iApply sem_typed_Sclosure. iIntros (σ).
     iApply sem_typed_sub_nil.
     rewrite - {1} (app_nil_r []). 
     iApply sem_typed_ufun; solve_sidecond. simpl.
     rewrite - [[("g", _); ("f", _)]]app_nil_r. 
     iApply sem_typed_afun; solve_sidecond. simpl.
-    set Γ₂ := [("g", τ -{ ⟨ρ.1,⟩ }-> ());
-               ("f", ((τ -{ ⟨ρ.1,⟩ }-> ()) → List τ -{ ⟨ρ.1,⟩ }-∘ ())%T)].
+    set Γ₂ := [("g", τ -{ σ }-> ());
+               ("f", ((τ -{ σ }-> ()) → List τ -{ σ }-∘ ())%T)].
     iApply (sem_typed_match_list _ Γ₂); solve_sidecond.
     - iApply sem_typed_sub_nil. rewrite - !/Γ₂.
       iApply (sem_typed_var Γ₂).
@@ -222,17 +222,17 @@ Section typing.
       iApply sem_typed_unit.
     - iApply sem_typed_seq.
       + iApply sem_typed_swap_third. iApply sem_typed_swap_second. 
-        iApply sem_typed_app_os; last (iApply sem_typed_sub_nil; iApply sem_typed_var).
+        iApply sem_typed_app; last (iApply sem_typed_sub_nil; iApply sem_typed_var).
         iApply sem_typed_contraction; solve_sidecond.
         simpl. iApply sem_typed_sub_ty; [iApply ty_le_u2aarr|].
         iApply sem_typed_sub_nil; iApply sem_typed_var.
       + iApply sem_typed_swap_second. rewrite -/Γ₂.
-        do 2 (iApply sem_typed_app_os;
+        do 2 (iApply sem_typed_app;
           last (iApply sem_typed_sub_nil; iApply sem_typed_var)).
         iApply sem_typed_sub_nil.
         iApply sem_typed_sub_ty. 
         { iApply ty_le_trans; [|iApply ty_le_u2aarr].
-          iApply ty_le_uarr. { simpl. iApply sigs_le_nil. }
+          iApply ty_le_uarr. { simpl. iApply sig_le_nil. }
           iApply ty_le_refl. iApply ty_le_refl. }
         iApply sem_typed_var.
   Qed.
@@ -275,7 +275,7 @@ Section typing.
       rewrite -/q.
       iApply (sem_typed_seq _ [x]). 
       { iApply sem_typed_replace_cpy; iApply sem_typed_var. }
-      iApply sem_typed_app_os; [iApply sem_typed_var|iApply sem_typed_unit].
+      iApply sem_typed_app; [iApply sem_typed_var|iApply sem_typed_unit].
   Qed.
 
   Definition resume_task_typed :
@@ -291,13 +291,13 @@ Section typing.
     set v := ("v", '! α).
     iApply sem_typed_ufun; solve_sidecond. simpl.
     set k := ("k", '! α ⊸ ()).
-    iApply (sem_typed_app_os _ [add]). 
+    iApply (sem_typed_app _ [add]). 
     { iApply sem_typed_sub_ty; [iApply ty_le_u2aarr|].
       iApply sem_typed_var. }
     replace ([k; v; add]) with ([k;v] ++ [add]) by done.
     iApply sem_typed_afun; solve_sidecond. simpl.
     iApply sem_typed_swap_second.
-    iApply sem_typed_app_os; iApply sem_typed_var.
+    iApply sem_typed_app; iApply sem_typed_var.
   Qed.
 
   Definition runner_typed :
@@ -313,20 +313,20 @@ Section typing.
     iApply sem_typed_contraction; solve_sidecond.
     set q := ("q", Queue).
     iApply (sem_typed_let _ [q; main]); solve_sidecond.
-    { iApply sem_typed_app_os; [|iApply sem_typed_var].
+    { iApply sem_typed_app; [|iApply sem_typed_var].
       iApply sem_typed_sub_ty; [iApply ty_le_u2aarr|].
       iApply sem_typed_val. iApply add_typed. }
     set add := ("add", add_ty).
     iApply sem_typed_swap_second. 
     iApply (sem_typed_let _ [add; main]); solve_sidecond. 
-    { rewrite /next. iApply sem_typed_app_os; [|iApply sem_typed_var].
+    { rewrite /next. iApply sem_typed_app; [|iApply sem_typed_var].
       iApply sem_typed_sub_ty; [iApply ty_le_u2aarr|].
       iApply sem_typed_val. iApply next_typed. }
     set next := ("next", next_ty).
     iApply sem_typed_swap_second. 
     iApply sem_typed_contraction; solve_sidecond.
     iApply (sem_typed_let _ [add; next; main]); solve_sidecond.
-    { iApply sem_typed_app_os; [|iApply sem_typed_var].
+    { iApply sem_typed_app; [|iApply sem_typed_var].
       iApply sem_typed_sub_ty; [iApply ty_le_u2aarr|].
       iApply sem_typed_val. iApply resume_task_typed. }
     set resume_task := ("resume_task", resume_task_ty).
@@ -334,33 +334,33 @@ Section typing.
     iApply (sem_typed_let _ [main]); solve_sidecond.
     - assert (Hrw : [resume_task;add;next;main] = [resume_task;add;next] ++ [main]) by done.
       rewrite Hrw. clear Hrw.
-      iApply (sem_typed_ufun_poly_rec _ _ _ _ _ (λ β, Promise ('! β)) (λ _, ⟨⟩%R) (λ β, (() -{ asig }-∘ '! β) ⊸ ())); 
+      iApply (sem_typed_ufun_poly_rec _ _ _ _ _ (λ β, Promise ('! β)) (λ _, ⊥) (λ β, (() -{ asig }-∘ '! β) ⊸ ())); 
         solve_sidecond. simpl.
      iIntros (β) "/=". 
      set promise := ("promise", Promise ('! β)).
-     set fulfill := ("fulfill", ∀T: β',, Promise ('! β') → (() -{ asig }-∘ '! β') ⊸ ()).
+     set fulfill := ("fulfill", ∀T: β', Promise ('! β') → (() -{ asig }-∘ '! β') ⊸ ()).
      rewrite -(app_nil_r [promise;fulfill;resume_task;add;next]).
      iApply sem_typed_afun; solve_sidecond. simpl.
      set comp := ("comp", () -{ asig }-∘ '! β)%T.
      replace ([comp; promise; fulfill; resume_task; add;next]) with
              ([comp] ++ [promise; fulfill; resume_task; add;next]) by done.
-     set A := λ (θ : sem_sig Σ) α, ( () -{ ⟨ θ, ⟩ }-∘ '! α ) + Promise ('! α).
+     set A := λ (θ : sem_sig Σ) α, ( () -{ θ }-∘ '! α ) + Promise ('! α).
      set B := (λ (θ : sem_sig Σ) α, Promise ('! α) + '! α).
-     iApply (sem_typed_deep_try_os' _ [] _ _ _ _ _ _ _ A B _ _ ⊥); solve_sidecond.
-     + iApply sem_typed_app_os; [iApply sem_typed_sub_nil; iApply sem_typed_var|].
+     iApply (sem_typed_deep_try _ [] _ _ _ _ _ _ _ A B _ _ ⊥); solve_sidecond.
+     + iApply sem_typed_app; [iApply sem_typed_sub_nil; iApply sem_typed_var|].
        iApply sem_typed_sub_nil. iApply sem_typed_unit. 
      + iIntros (β').
        iApply sem_typed_swap_third. iApply sem_typed_weaken.
        iApply sem_typed_swap_fourth. iApply sem_typed_weaken.
-       set k := ("k", B (μ∀TS: θ, α0, A θ α0 ⇒ B θ α0)%R β' ⊸ ()).
+       set k := ("k", B (μ∀TS: θ, α0, A θ α0 ⇒ B θ α0)%S β' ⊸ ()).
        rewrite -/k -/fulfill -/add -/next.
        iApply (sem_typed_match _ [k; fulfill; add; next]); solve_sidecond; first iApply sem_typed_var.
-       * simpl. set x := ("x", () -{ ⟨ μ∀TS: θ, α0, A θ α0 ⇒ B θ α0, ⟩ }-∘ '! β').
+       * simpl. set x := ("x", () -{ μ∀TS: θ, α0, A θ α0 ⇒ B θ α0 }-∘ '! β').
          iApply (sem_typed_let _ [x; k; fulfill; add; next] _ _ _ _ (Promise ('! β'))); solve_sidecond.
          { iApply sem_typed_alloc_cpy. iApply sem_typed_right_inj. iApply sem_typed_nil. }
          set new_prom := ("new_prom", Promise ('! β')).
          iApply (sem_typed_seq _ [new_prom; k; next]).
-         ** iApply (sem_typed_app_os _ [new_prom; k; add; next]).
+         ** iApply (sem_typed_app _ [new_prom; k; add; next]).
             { iApply sem_typed_swap_third.
               iApply sem_typed_sub_ty; [iApply ty_le_u2aarr|iApply sem_typed_var]. }
             iApply sem_typed_swap_fourth. iApply sem_typed_swap_second.
@@ -370,13 +370,13 @@ Section typing.
                           [fulfill; x; new_prom] ++ [new_prom; k; add; next]) by done.
             rewrite Hrw. clear Hrw.
             iApply sem_typed_afun; solve_sidecond. simpl.
-            do 2 (iApply sem_typed_swap_second; iApply sem_typed_app_os; [|iApply sem_typed_var]).
+            do 2 (iApply sem_typed_swap_second; iApply sem_typed_app; [|iApply sem_typed_var]).
             rewrite -/asig.
             iApply sem_typed_sub_ty; [iApply ty_le_u2aarr|]. 
             set C := (λ β, Promise ('! β) → (() -{ asig }-∘ '! β) ⊸ ())%T.
             rewrite -/(C β').
             iApply sem_typed_TApp; first solve_copy. iApply sem_typed_var.
-         ** iApply (sem_typed_app_os _ [k]); [iApply sem_typed_var|].
+         ** iApply (sem_typed_app _ [k]); [iApply sem_typed_var|].
             iApply sem_typed_swap_third. iApply sem_typed_weaken.
             iApply sem_typed_left_inj. iApply sem_typed_var.
       * simpl.
@@ -395,7 +395,7 @@ Section typing.
            iApply (sem_typed_seq _ [v; k]).
            {  iApply sem_typed_replace_cpy; [iApply sem_typed_var|].
              iApply sem_typed_left_inj. iApply sem_typed_var. }
-           iApply sem_typed_app_os; [iApply sem_typed_var|].
+           iApply sem_typed_app; [iApply sem_typed_var|].
            iApply sem_typed_right_inj. iApply sem_typed_var.
         ** simpl. set ks := ("ks", List ('! β' ⊸ ())).
            iApply (sem_typed_seq _ [next] _ _ _ (Status ('! β'))).
@@ -407,9 +407,9 @@ Section typing.
                assert (Hrw : [k; p; next] = [k] ++ [p;next]) by done.
                rewrite Hrw. clear Hrw.
                iApply sem_typed_afun; solve_sidecond. simpl.
-               iApply sem_typed_app_os; [iApply sem_typed_var|].
+               iApply sem_typed_app; [iApply sem_typed_var|].
                iApply sem_typed_right_inj. iApply sem_typed_var.
-           *** iApply sem_typed_app_os; [|iApply sem_typed_unit].
+           *** iApply sem_typed_app; [|iApply sem_typed_unit].
                iApply sem_typed_sub_ty; [iApply ty_le_u2aarr|iApply sem_typed_var].
     + simpl. 
       iApply sem_typed_swap_third. iApply sem_typed_weaken.
@@ -432,21 +432,21 @@ Section typing.
         ** iApply sem_typed_replace_cpy; [iApply sem_typed_var|].
            iApply sem_typed_left_inj. iApply sem_typed_var.
         ** iApply (sem_typed_seq _ [next]).
-           2: { iApply sem_typed_app_os; [|iApply sem_typed_unit].
+           2: { iApply sem_typed_app; [|iApply sem_typed_unit].
                 iApply sem_typed_sub_ty; [iApply ty_le_u2aarr|iApply sem_typed_var]. }
            iApply sem_typed_swap_second.
-           iApply (sem_typed_app_os _ _ _ _ _ (List ('! β ⊸ ())) _ ()); [|iApply sem_typed_var].
-           iApply (sem_typed_app_os _ [next] _ _ _ (('! β ⊸ ()) → ())%T).
-           2: { iApply sem_typed_app_os; [|iApply sem_typed_var]. 
+           iApply (sem_typed_app _ _ _ _ _ (List ('! β ⊸ ())) _ ()); [|iApply sem_typed_var].
+           iApply (sem_typed_app _ [next] _ _ _ (('! β ⊸ ()) → ())%T).
+           2: { iApply sem_typed_app; [|iApply sem_typed_var]. 
                 iApply sem_typed_sub_ty; [iApply ty_le_u2aarr|].
                 set C := λ β, ('! β → ('! β ⊸ ()) → ())%T. rewrite -/(C β). simpl.
                 iApply sem_typed_TApp; first solve_sidecond. iApply sem_typed_var. }
            iApply sem_typed_sub_ty; [iApply ty_le_u2aarr|].
-           set C := (λ (θ : sem_sigs Σ), (('! β ⊸ ()) -{ ⟨θ.1,⟩ }-> ()) → List ('! β ⊸ ()) -{ ⟨θ.1,⟩ }-∘ ())%T.
-           rewrite -/(C ⟨⟩%R).
+           set C := (λ (θ : sem_sig Σ), (('! β ⊸ ()) -{ θ }-> ()) → List ('! β ⊸ ()) -{ θ }-∘ ())%T.
+           rewrite -/(C ⊥).
            iApply sem_typed_SApp; first solve_copy. 
            iApply sem_typed_val. iApply iter_typed.
-  - set fulfill := ("fulfill", ∀T: α,, Promise ('! α) → (() -{ asig }-∘ '! α) ⊸ ()).
+  - set fulfill := ("fulfill", ∀T: α, Promise ('! α) → (() -{ asig }-∘ '! α) ⊸ ()).
     iApply (sem_typed_let _ [fulfill; main]); solve_sidecond.
     { iApply (sem_typed_alloc_cpy _ _ _ _ (Status ('! α))). 
       iApply sem_typed_right_inj. iApply sem_typed_nil. }
@@ -454,8 +454,8 @@ Section typing.
     iApply sem_typed_contraction; solve_sidecond.
     iApply sem_typed_swap_third. iApply sem_typed_swap_second. iApply sem_typed_swap_fourth.
     iApply (sem_typed_seq _ [pmain]).
-    + iApply (sem_typed_app_os _ _ _ _ _ _ _ ()); [|iApply sem_typed_var]. 
-      iApply sem_typed_app_os; [|iApply sem_typed_var]. 
+    + iApply (sem_typed_app _ _ _ _ _ _ _ ()); [|iApply sem_typed_var]. 
+      iApply sem_typed_app; [|iApply sem_typed_var]. 
       iApply sem_typed_sub_ty; [iApply ty_le_u2aarr|].
       set C := (λ α, Promise ('! α) → (() -{ asig }-∘ '! α) ⊸ ())%T.
       rewrite -/(C α).
