theories/logic/compatibility.v
@@ -40,7 +40,7 @@ Section compatibility.
   Context `{!heapGS Σ}.
   
   Lemma sem_typed_val Γ τ v : 
-    ⊨ᵥ v : τ -∗ Γ ⊨ v : ⟨⟩ : τ ⊨ Γ.
+    ⊨ᵥ v : τ -∗ Γ ⊨ v : ⊥ : τ ⊨ Γ.
   Proof.
     iIntros "#Hv !# %vs HΓ /=".
     iApply ewp_value. iFrame.
@@ -51,42 +51,42 @@ Section compatibility.
   (* Base rules *)
   
   Lemma sem_typed_unit Γ : 
-    ⊢ Γ ⊨ #() : ⟨⟩ : () ⊨ Γ.
+    ⊢ Γ ⊨ #() : ⊥ : () ⊨ Γ.
   Proof.
     iIntros (vs) "!# HΓ₁ //=". iApply ewp_value. by iFrame.
   Qed.
   
   Lemma sem_typed_bool Γ (b : bool) : 
-    ⊢ Γ ⊨ #b : ⟨⟩ : 𝔹 ⊨ Γ.
+    ⊢ Γ ⊨ #b : ⊥ : 𝔹 ⊨ Γ.
   Proof.
     iIntros (vs) "!# HΓ₁ //=". iApply ewp_value. 
     iSplitR; first (iExists b); done.
   Qed.
   
   Lemma sem_typed_int Γ (i : Z) : 
-    ⊢ Γ ⊨ #i : ⟨⟩ : ℤ ⊨ Γ.
+    ⊢ Γ ⊨ #i : ⊥ : ℤ ⊨ Γ.
   Proof.
     iIntros (vs) "!# HΓ₁ //=". iApply ewp_value. 
     iSplitR; first (iExists i); done.
   Qed.
   
   Lemma sem_typed_var Γ x τ : 
-    ⊢ (x, τ) :: Γ ⊨ x : ⟨⟩ : τ ⊨ Γ.
+    ⊢ (x, τ) :: Γ ⊨ x : ⊥ : τ ⊨ Γ.
   Proof.
     iIntros (vs) "!# /= [%v (%Hrw & Hτ & HΓ₁)] /=". 
     rewrite Hrw. iApply ewp_value. iFrame.
   Qed.
 
   Lemma sem_typed_void_in_env Γ₁ Γ₂ e x τ : 
-    ⊢ (x, Void) :: Γ₁ ⊨ e : ⟨⟩ : τ ⊨ Γ₂.
+    ⊢ (x, Void) :: Γ₁ ⊨ e : ⊥ : τ ⊨ Γ₂.
   Proof.
     iIntros (vs) "!# /= [%v (%Hrw & [] & _)] /=". 
   Qed.
 
-  Lemma sem_typed_closure f x e τ ρs κ :
+  Lemma sem_typed_closure f x e τ σ κ :
     match f with BNamed f => BNamed f ≠ x | BAnon => True end →
-    (x, τ) ::? (f, τ -{ ρs }-> κ) ::? [] ⊨ e : ρs : κ ⊨ [] -∗ 
-    ⊨ᵥ (rec: f x := e) : (τ -{ ρs }-> κ).
+    (x, τ) ::? (f, τ -{ σ }-> κ) ::? [] ⊨ e : σ : κ ⊨ [] -∗ 
+    ⊨ᵥ (rec: f x := e) : (τ -{ σ }-> κ).
   Proof.
       iIntros (?) "#He !#". iLöb as "IH".
       iIntros "%v !# Hτ /=". 
@@ -106,9 +106,9 @@ Section compatibility.
         intros ?; simplify_eq.
   Qed.
 
-  Lemma sem_typed_Tclosure e τ ρs :
-    (∀ α, ⊨ e : ρs : τ α) -∗ 
-    ⊨ᵥ (Λ: e) : (∀T: α, ρs , τ α).
+  Lemma sem_typed_Tclosure e τ :
+    (∀ α, ⊨ e : ⊥ : τ α) -∗ 
+    ⊨ᵥ (Λ: e) : (∀T: α, τ α).
   Proof.
     iIntros "#He !# %u !#". ewp_pure_steps.
     rewrite - {2} [e]subst_map_empty.
@@ -118,19 +118,19 @@ Section compatibility.
   Qed.
 
   (* Signature abstraction and application *)
-  Lemma sem_typed_Rclosure e C : 
-    (∀ θ, ⊨ e : ⟨⟩ : C θ) -∗
-    ⊨ᵥ (Λ: e) : (∀R: θ , C θ)%T.
+  Lemma sem_typed_Sclosure e C : 
+    (∀ θ, ⊨ e : ⊥ : C θ) -∗
+    ⊨ᵥ (Λ: e) : (∀S: θ , C θ)%T.
   Proof.
-    iIntros "#He !# %ρ !# /=".
+    iIntros "#He !# %σ !# /=".
     ewp_pure_steps. rewrite - {2} [e]subst_map_empty. 
     iApply (ewp_pers_mono with "[He]"); [by iApply "He"|].
     iIntros "!# % [$ _] //=". 
   Qed.
 
-  Lemma sem_typed_closure_to_unrestricted x e τ ρs κ :
-    ⊨ᵥ (λ: x, e) : (τ -{ ρs }-∘ κ) -∗
-    ⊨ᵥ (λ: x, e) : (τ -{ ρs }-> κ).
+  Lemma sem_typed_closure_to_unrestricted x e τ σ κ :
+    ⊨ᵥ (λ: x, e) : (τ -{ σ }-∘ κ) -∗
+    ⊨ᵥ (λ: x, e) : (τ -{ σ }-> κ).
   Proof. 
     iIntros "#He !# %w !# Hτ". 
     iSpecialize ("He" $! w).
@@ -139,83 +139,82 @@ Section compatibility.
 
   (* Subsumption rule *)
   
-  Lemma sem_typed_sub Γ₁ Γ₁' Γ₂ Γ₂' e ρs ρs' τ τ':
+  Lemma sem_typed_sub Γ₁ Γ₁' Γ₂ Γ₂' e σ σ' τ τ':
     Γ₁  ≤E Γ₁' -∗
     Γ₂' ≤E Γ₂ -∗
-    ρs' ≤Rs ρs -∗ 
+    σ'  ≤S σ -∗ 
     τ'  ≤T τ -∗
-    Γ₁' ⊨ e : ρs' : τ' ⊨ Γ₂' -∗ Γ₁ ⊨ e : ρs : τ ⊨ Γ₂.
+    Γ₁' ⊨ e : σ' : τ' ⊨ Γ₂' -∗ Γ₁ ⊨ e : σ : τ ⊨ Γ₂.
   Proof.
-    iIntros "#HΓ₁le #HΓ₂le [#Hρle₁ #Hρle₂] #Hτle #He !# %vs HΓ₁ //=".
+    iIntros "#HΓ₁le #HΓ₂le #Hσle #Hτle #He !# %vs HΓ₁ //=".
     iDestruct ("HΓ₁le" with "HΓ₁") as "HΓ₁'".
-    iApply ewp_os_prot_mono; [iApply "Hρle₁"|].
-    iApply ewp_ms_prot_mono; [iApply "Hρle₂"|].
+    iApply ewp_os_prot_mono; [iApply "Hσle"|].
     iApply (ewp_pers_mono with "[HΓ₁']"); first (by iApply "He").
     iIntros "!# % [Hτ HΓ₂] //= !>".
     iSplitL "Hτ"; [by iApply "Hτle"|by iApply "HΓ₂le"].
   Qed. 
   
   (* Convenient Subsumption rules *)
-  Lemma sem_typed_sub_ty τ' τ Γ₁ Γ₂ e ρs :
+  Lemma sem_typed_sub_ty τ' τ Γ₁ Γ₂ e σ :
   τ' ≤T τ -∗
-  (Γ₁ ⊨ e : ρs : τ' ⊨ Γ₂) -∗ Γ₁ ⊨ e : ρs : τ ⊨ Γ₂.
+  (Γ₁ ⊨ e : σ : τ' ⊨ Γ₂) -∗ Γ₁ ⊨ e : σ : τ ⊨ Γ₂.
   Proof.
     iIntros "#Hτ".
-    iApply (sem_typed_sub Γ₁ Γ₁ Γ₂ Γ₂ _ ρs ρs);
-      (iApply sigs_le_refl || iApply env_le_refl || done). 
+    iApply (sem_typed_sub Γ₁ Γ₁ Γ₂ Γ₂ _ σ σ);
+      (iApply sig_le_refl || iApply env_le_refl || done). 
   Qed.
 
-  Lemma sem_typed_sub_sig ρs ρs' Γ₁ Γ₂ e τ :
-    ρs' ≤Rs ρs -∗
-    (Γ₁ ⊨ e : ρs' : τ ⊨ Γ₂) -∗ Γ₁ ⊨ e : ρs : τ ⊨ Γ₂.
+  Lemma sem_typed_sub_sig σ σ' Γ₁ Γ₂ e τ :
+    σ' ≤S σ -∗
+    (Γ₁ ⊨ e : σ' : τ ⊨ Γ₂) -∗ Γ₁ ⊨ e : σ : τ ⊨ Γ₂.
   Proof.
-    iIntros "#Hρ".
-    iApply (sem_typed_sub Γ₁ Γ₁ Γ₂ Γ₂ _ ρs ρs' τ τ);
-      (iApply sigs_le_refl || iApply env_le_refl || iApply ty_le_refl || done).
+    iIntros "#Hσ".
+    iApply (sem_typed_sub Γ₁ Γ₁ Γ₂ Γ₂ _ σ σ' τ τ);
+      (iApply env_le_refl || iApply ty_le_refl || done).
   Qed.
 
-  Lemma sem_typed_sub_nil Γ₁ Γ₂ e τ ρs :
-    (Γ₁ ⊨ e : ⟨⟩ : τ ⊨ Γ₂) -∗ Γ₁ ⊨ e : ρs : τ ⊨ Γ₂.
-  Proof. iApply sem_typed_sub_sig. iApply sigs_le_nil. Qed.
+  Lemma sem_typed_sub_nil Γ₁ Γ₂ e τ σ :
+    (Γ₁ ⊨ e : ⊥ : τ ⊨ Γ₂) -∗ Γ₁ ⊨ e : σ : τ ⊨ Γ₂.
+  Proof. iApply sem_typed_sub_sig. iApply sig_le_nil. Qed.
   
-  Lemma sem_typed_sub_env Γ₁ Γ₁' Γ₂ e ρs τ :
+  Lemma sem_typed_sub_env Γ₁ Γ₁' Γ₂ e σ τ :
     Γ₁ ≤E Γ₁' -∗
-    (Γ₁' ⊨ e : ρs : τ ⊨ Γ₂) -∗ Γ₁ ⊨ e : ρs : τ ⊨ Γ₂.
+    (Γ₁' ⊨ e : σ : τ ⊨ Γ₂) -∗ Γ₁ ⊨ e : σ : τ ⊨ Γ₂.
   Proof.
     iIntros "#HΓ₁".
-    iApply (sem_typed_sub Γ₁ Γ₁' Γ₂ Γ₂ _ ρs ρs τ τ);
-      (iApply sigs_le_refl || iApply env_le_refl || iApply ty_le_refl || done).
+    iApply (sem_typed_sub Γ₁ Γ₁' Γ₂ Γ₂ _ σ σ τ τ);
+      (iApply sig_le_refl || iApply env_le_refl || iApply ty_le_refl || done).
   Qed.
 
-  Lemma sem_typed_sub_env_final Γ₁ Γ₂ Γ₂' e ρs τ :
+  Lemma sem_typed_sub_env_final Γ₁ Γ₂ Γ₂' e σ τ :
     Γ₂' ≤E Γ₂ -∗
-    (Γ₁ ⊨ e : ρs : τ ⊨ Γ₂') -∗ Γ₁ ⊨ e : ρs : τ ⊨ Γ₂.
+    (Γ₁ ⊨ e : σ : τ ⊨ Γ₂') -∗ Γ₁ ⊨ e : σ : τ ⊨ Γ₂.
   Proof.
     iIntros "#HΓ₂".
-    iApply (sem_typed_sub Γ₁ Γ₁ Γ₂ Γ₂' _ ρs ρs τ τ);
-      (iApply sigs_le_refl || iApply env_le_refl || iApply ty_le_refl || done).
+    iApply (sem_typed_sub Γ₁ Γ₁ Γ₂ Γ₂' _ σ σ τ τ);
+      (iApply sig_le_refl || iApply env_le_refl || iApply ty_le_refl || done).
   Qed.
 
-  Lemma sem_typed_swap_second Γ₁ Γ₂ x y e ρs τ₁ τ₂ κ :
-    ((y, τ₂) :: (x, τ₁) :: Γ₁ ⊨ e : ρs : κ ⊨ Γ₂) -∗ 
-    ((x, τ₁) :: (y, τ₂) :: Γ₁ ⊨ e : ρs : κ ⊨ Γ₂).
+  Lemma sem_typed_swap_second Γ₁ Γ₂ x y e σ τ₁ τ₂ κ :
+    ((y, τ₂) :: (x, τ₁) :: Γ₁ ⊨ e : σ : κ ⊨ Γ₂) -∗ 
+    ((x, τ₁) :: (y, τ₂) :: Γ₁ ⊨ e : σ : κ ⊨ Γ₂).
   Proof.
     iIntros "He".
     iApply sem_typed_sub_env; [iApply env_le_swap_second|iApply "He"].
   Qed.
 
-  Lemma sem_typed_swap_third Γ₁ Γ₂ x y z e ρs τ₁ τ₂ τ₃ κ :
-    ((z, τ₃) :: (x, τ₁) :: (y, τ₂) :: Γ₁ ⊨ e : ρs : κ ⊨ Γ₂) -∗ 
-    ((x, τ₁) :: (y, τ₂) :: (z, τ₃) :: Γ₁ ⊨ e : ρs : κ ⊨ Γ₂).
+  Lemma sem_typed_swap_third Γ₁ Γ₂ x y z e σ τ₁ τ₂ τ₃ κ :
+    ((z, τ₃) :: (x, τ₁) :: (y, τ₂) :: Γ₁ ⊨ e : σ : κ ⊨ Γ₂) -∗ 
+    ((x, τ₁) :: (y, τ₂) :: (z, τ₃) :: Γ₁ ⊨ e : σ : κ ⊨ Γ₂).
   Proof.
     iIntros "He".
     iApply sem_typed_sub_env; [|iApply "He"].
     iApply env_le_trans; iApply env_le_swap_third.
   Qed.
 
-  Lemma sem_typed_swap_fourth Γ₁ Γ₂ x y z z' e ρs τ₁ τ₂ τ₃ τ₄ κ :
-    ((z', τ₄) :: (x, τ₁) :: (y, τ₂) :: (z, τ₃) :: Γ₁ ⊨ e : ρs : κ ⊨ Γ₂) -∗ 
-    ((x, τ₁) :: (y, τ₂) :: (z, τ₃) :: (z', τ₄) :: Γ₁ ⊨ e : ρs : κ ⊨ Γ₂).
+  Lemma sem_typed_swap_fourth Γ₁ Γ₂ x y z z' e σ τ₁ τ₂ τ₃ τ₄ κ :
+    ((z', τ₄) :: (x, τ₁) :: (y, τ₂) :: (z, τ₃) :: Γ₁ ⊨ e : σ : κ ⊨ Γ₂) -∗ 
+    ((x, τ₁) :: (y, τ₂) :: (z, τ₃) :: (z', τ₄) :: Γ₁ ⊨ e : σ : κ ⊨ Γ₂).
   Proof.
     iIntros "He".
     iApply sem_typed_sub_env; [|iApply "He"].
@@ -223,44 +222,44 @@ Section compatibility.
     iApply env_le_swap_fourth.
   Qed.
 
-  Lemma sem_typed_swap_env_singl Γ₁ Γ₂ x e ρs τ κ :
-    (Γ₁ ++ [(x, τ)] ⊨ e : ρs : κ ⊨ Γ₂) -∗ 
-    ((x, τ) :: Γ₁ ⊨ e : ρs : κ ⊨ Γ₂). 
+  Lemma sem_typed_swap_env_singl Γ₁ Γ₂ x e σ τ κ :
+    (Γ₁ ++ [(x, τ)] ⊨ e : σ : κ ⊨ Γ₂) -∗ 
+    ((x, τ) :: Γ₁ ⊨ e : σ : κ ⊨ Γ₂). 
   Proof.
     iIntros "He".
     iApply sem_typed_sub_env; [|iApply "He"].
     iApply env_le_swap_env_singl.
   Qed.
 
-  Lemma sem_typed_contraction Γ₁ Γ₂ x e ρs τ κ :
+  Lemma sem_typed_contraction Γ₁ Γ₂ x e σ τ κ :
     copy_ty τ -∗
-    (x, τ) :: (x, τ) :: Γ₁ ⊨ e : ρs : κ ⊨ Γ₂ -∗ 
-    (x, τ) :: Γ₁ ⊨ e : ρs : κ ⊨ Γ₂.
+    (x, τ) :: (x, τ) :: Γ₁ ⊨ e : σ : κ ⊨ Γ₂ -∗ 
+    (x, τ) :: Γ₁ ⊨ e : σ : κ ⊨ Γ₂.
   Proof.
     iIntros "#τ He".
     iApply sem_typed_sub_env; 
       [by iApply env_le_copy_contraction|iApply "He"].
   Qed.
 
-  Lemma sem_typed_weaken Γ₁ Γ₂ x e ρs τ κ :
-    (Γ₁ ⊨ e : ρs : κ ⊨ Γ₂) -∗ ((x, τ) :: Γ₁ ⊨ e : ρs : κ ⊨ Γ₂).
+  Lemma sem_typed_weaken Γ₁ Γ₂ x e σ τ κ :
+    (Γ₁ ⊨ e : σ : κ ⊨ Γ₂) -∗ ((x, τ) :: Γ₁ ⊨ e : σ : κ ⊨ Γ₂).
   Proof.
     iIntros "He".
     iApply sem_typed_sub_env; [iApply env_le_weaken|iApply "He"].
   Qed.
 
-  Lemma sem_typed_frame_os Γ₁ e ρ x τ κ Γ₂:
-    Γ₁ ⊨ e : ⟨ ρ, ⟩ : κ ⊨ Γ₂ -∗
-    (x, τ) :: Γ₁ ⊨ e : ⟨ ρ, ⟩ : κ ⊨ (x, τ) :: Γ₂.
+  Lemma sem_typed_frame Γ₁ e σ x τ κ Γ₂:
+    Γ₁ ⊨ e : σ : κ ⊨ Γ₂ -∗
+    (x, τ) :: Γ₁ ⊨ e : σ : κ ⊨ (x, τ) :: Γ₂.
   Proof.
     iIntros "#He %vs !# (%v & %Hrw & Hτ & HΓ₁)".
     iApply (ewp_mono with "[HΓ₁]"); first (by iApply "He").
     iIntros (w) "[Hκ HΓ₂]". solve_env.
   Qed.
 
-  Lemma sem_typed_frame_env_os Γ₁ Γ' e ρ τ Γ₂ :
-    Γ₁ ⊨ e : ⟨ ρ, ⟩ : τ ⊨ Γ₂ -∗
-    Γ' ++ Γ₁ ⊨ e : ⟨ ρ, ⟩ : τ ⊨ Γ' ++ Γ₂.
+  Lemma sem_typed_frame_env Γ₁ Γ' e σ τ Γ₂ :
+    Γ₁ ⊨ e : σ : τ ⊨ Γ₂ -∗
+    Γ' ++ Γ₁ ⊨ e : σ : τ ⊨ Γ' ++ Γ₂.
   Proof.
     iIntros "#He %vs !# HΓ'Γ₁".
     iDestruct (env_sem_typed_app with "HΓ'Γ₁") as "[HΓ' HΓ₁]".
@@ -272,23 +271,12 @@ Section compatibility.
     iIntros (w) "[$ HΓ] !>". solve_env.
   Qed.
 
-  Lemma sem_typed_frame_ms Γ₁ e ρs x τ κ Γ₂:
-    copy_ty τ -∗
-    Γ₁ ⊨ e : ρs : κ ⊨ Γ₂ -∗
-    (x, τ) :: Γ₁ ⊨ e : ρs : κ ⊨ (x, τ) :: Γ₂.
-  Proof.
-    iIntros "#Hcpy #He %vs !# (%v & %Hrw & Hτ & HΓ₁)".
-    iDestruct ("Hcpy" with "Hτ") as "#Hτ'".
-    iApply (ewp_pers_mono with "[HΓ₁]"); first (by iApply "He").
-    iIntros "!# % [Hκ HΓ₂]". solve_env.
-  Qed.
-
   (* λ-calculus rules *)
 
-  Lemma sem_typed_afun Γ₁ Γ₂ x e τ ρs κ: 
+  Lemma sem_typed_afun Γ₁ Γ₂ x e τ σ κ: 
     x ∉ (env_dom Γ₁) → x ∉ (env_dom Γ₂) →
-    (x,τ) ::? Γ₁ ⊨ e : ρs : κ ⊨ [] -∗
-    Γ₁ ++ Γ₂ ⊨ (λ: x, e) : ⟨⟩ : (τ -{ ρs }-∘ κ) ⊨ Γ₂.
+    (x,τ) ::? Γ₁ ⊨ e : σ : κ ⊨ [] -∗
+    Γ₁ ++ Γ₂ ⊨ (λ: x, e) : ⊥ : (τ -{ σ }-∘ κ) ⊨ Γ₂.
   Proof.
     iIntros (??) "#He !# %vs HΓ₁₂ //=".
     iDestruct (env_sem_typed_app with "HΓ₁₂") as "[HΓ₁ HΓ₂]".
@@ -299,12 +287,12 @@ Section compatibility.
     destruct x; solve_env. 
   Qed.
 
-  Lemma sem_typed_ufun Γ₁ Γ₂ f x e τ ρs κ:
+  Lemma sem_typed_ufun Γ₁ Γ₂ f x e τ σ κ:
     x ∉ (env_dom Γ₁) → f ∉ (env_dom Γ₁) → 
     match f with BNamed f => BNamed f ≠ x | BAnon => True end →
     copy_env Γ₁ -∗
-    (x, τ) ::? (f, τ -{ ρs }-> κ) ::? Γ₁ ⊨ e : ρs : κ ⊨ [] -∗
-    Γ₁ ++ Γ₂ ⊨ (rec: f x := e) : ⟨⟩ : (τ -{ ρs }-> κ) ⊨ Γ₂.
+    (x, τ) ::? (f, τ -{ σ }-> κ) ::? Γ₁ ⊨ e : σ : κ ⊨ [] -∗
+    Γ₁ ++ Γ₂ ⊨ (rec: f x := e) : ⊥ : (τ -{ σ }-> κ) ⊨ Γ₂.
   Proof.
     iIntros (???) "#HcpyΓ₁ #He !# %vs HΓ₁₂ //=".
     ewp_pure_steps.
@@ -332,12 +320,12 @@ Section compatibility.
       by do 2 (rewrite -env_sem_typed_insert; last done).
   Qed.
 
-  Lemma sem_typed_ufun_poly_rec Γ₁ Γ₂ f x e τ ρs κ:
+  Lemma sem_typed_ufun_poly_rec Γ₁ Γ₂ f x e τ σ κ:
     x ∉ (env_dom Γ₁) → f ∉ (env_dom Γ₁) → 
     match x with BNamed x => BNamed x ≠ f | BAnon => True end →
     copy_env Γ₁ -∗
-    (∀ ι, (x, τ ι) ::? (f, ∀T: α,, τ α -{ ρs α }-> κ α) ::? Γ₁ ⊨ e : ρs ι : κ ι ⊨ []) -∗
-    Γ₁ ++ Γ₂ ⊨ (rec: f <> := λ: x, e) : ⟨⟩ : (∀T: α,, τ α -{ ρs α }-> κ α) ⊨ Γ₂.
+    (∀ ι, (x, τ ι) ::? (f, ∀T: α, τ α -{ σ α }-> κ α) ::? Γ₁ ⊨ e : σ ι : κ ι ⊨ []) -∗
+    Γ₁ ++ Γ₂ ⊨ (rec: f <> := λ: x, e) : ⊥ : (∀T: α, τ α -{ σ α }-> κ α) ⊨ Γ₂.
   Proof.
     iIntros (???) "#HcpyΓ₁ #He !# %vs HΓ₁₂ //=".
     ewp_pure_steps. rewrite env_sem_typed_app. 
@@ -367,11 +355,11 @@ Section compatibility.
       + iIntros "!# % [$ _] //=".
   Qed.
 
-  Lemma sem_typed_let Γ₁ Γ₂ Γ₃ x e₁ e₂ τ ρs κ: 
+  Lemma sem_typed_let Γ₁ Γ₂ Γ₃ x e₁ e₂ τ σ κ: 
     x ∉ (env_dom Γ₂) → x ∉ (env_dom Γ₃) →
-    Γ₁ ⊨ e₁ : ρs : τ ⊨ Γ₂ -∗
-    (x, τ) :: Γ₂ ⊨ e₂ : ρs : κ ⊨ Γ₃ -∗
-    Γ₁ ⊨ (let: x := e₁ in e₂) : ρs : κ ⊨ Γ₃.
+    Γ₁ ⊨ e₁ : σ : τ ⊨ Γ₂ -∗
+    (x, τ) :: Γ₂ ⊨ e₂ : σ : κ ⊨ Γ₃ -∗
+    Γ₁ ⊨ (let: x := e₁ in e₂) : σ : κ ⊨ Γ₃.
   Proof.
     iIntros (??) "#He₁ #He₂ !# %vs HΓ₁ /=".
     iApply (ewp_bind ([AppRCtx _])); first done. simpl.
@@ -383,68 +371,26 @@ Section compatibility.
     solve_env.
   Qed.
 
-  Lemma sem_typed_app Γ₁ Γ₂ Γ₃ e₁ e₂ τ ρs κ: 
-    copy_env Γ₃ -∗
-    Γ₂ ⊨ e₁ : ⟨ρs.1,⟩ : (τ -{ ρs }-∘ κ) ⊨ Γ₃ -∗
-    Γ₁ ⊨ e₂ : ρs : τ ⊨ Γ₂ -∗
-    Γ₁ ⊨ (e₁ e₂) : ρs : κ ⊨ Γ₃.
-  Proof.
-    iIntros "#Hcpy #He₁ #He₂ !# %vs HΓ₁ /=".
-    iApply (ewp_bind [AppRCtx _]); first done.
-    iApply (ewp_pers_mono with "[HΓ₁]"); first (by iApply "He₂").
-    iIntros "!# % [Hτ HΓ₂] !> /=".
-    iApply (ewp_bind [AppLCtx _]); first done.
-    iApply ewp_ms_prot_mono; [iApply sig_le_nil|].
-    iApply (ewp_mono with "[HΓ₂]"); first (by iApply "He₁").
-    iIntros "% [Hτκ HΓ₃'] !> /=".
-    iDestruct ("Hcpy" with "HΓ₃'") as "#HΓ₃".
-    iApply (ewp_pers_mono with "[Hτ Hτκ]"); first (by iApply "Hτκ").
-    iIntros "!# % $ !> //=".
-  Qed.
-
-  Lemma sem_typed_app_ms Γ₁ Γ₂ Γ₃ (x₁ x₂ : string) e₁ e₂ τ ρs κ: 
-    x₂ ∉ env_dom Γ₂ → x₂ ∉ env_dom Γ₃ → 
-    x₁ ∉ env_dom Γ₃ → x₁ ≠ x₂ →
-    copy_ty τ -∗ copy_env Γ₃ -∗
-    Γ₂ ⊨ e₁ : ρs : (τ -{ ρs }-∘ κ) ⊨ Γ₃ -∗
-    Γ₁ ⊨ e₂ : ρs : τ ⊨ Γ₂ -∗
-    Γ₁ ⊨ (e₁ e₂) : ρs : κ ⊨ Γ₃.
-  Proof.
-    iIntros (????) "#Hcpyτ #HcpyΓ₃ #He₁ #He₂ !# %vs HΓ₁ /=".
-    iApply (ewp_bind [AppRCtx _]); first done.
-    iApply (ewp_pers_mono with "[HΓ₁]"); first (by iApply "He₂").
-    iIntros "!# % [Hτ HΓ₂] !> /=".
-    iApply (ewp_bind [AppLCtx _]); first done.
-    iDestruct ("Hcpyτ" with "Hτ") as "#Hτ'".
-    iApply (ewp_pers_mono with "[HΓ₂]"); first (by iApply "He₁").
-    iIntros "!# % [Hτκ HΓ₃] !> /=".
-    iDestruct ("HcpyΓ₃" with "HΓ₃") as "#HΓ₃'".
-    iApply (ewp_pers_mono with "[Hτ' Hτκ]"); first (by iApply "Hτκ").
-    iIntros "!# % $ !> //=".
-  Qed.
-
-  Lemma sem_typed_app_os Γ₁ Γ₂ Γ₃ e₁ e₂ τ ρs κ: 
-    Γ₂ ⊨ e₁ : ⟨ρs.1,⟩ : (τ -{ ⟨ρs.1,⟩ }-∘ κ) ⊨ Γ₃ -∗
-    Γ₁ ⊨ e₂ : ρs : τ ⊨ Γ₂ -∗
-    Γ₁ ⊨ (e₁ e₂) : ρs : κ ⊨ Γ₃.
+  Lemma sem_typed_app Γ₁ Γ₂ Γ₃ e₁ e₂ τ σ κ: 
+    Γ₂ ⊨ e₁ : σ : (τ -{ σ }-∘ κ) ⊨ Γ₃ -∗
+    Γ₁ ⊨ e₂ : σ : τ ⊨ Γ₂ -∗
+    Γ₁ ⊨ (e₁ e₂) : σ : κ ⊨ Γ₃.
   Proof.
     iIntros "#He₁ #He₂ !# %vs HΓ₁ /=".
     iApply (ewp_bind [AppRCtx _]); first done.
     iApply (ewp_pers_mono with "[HΓ₁]"); first (by iApply "He₂").
     iIntros "!# % [Hτ HΓ₂] !> /=".
     iApply (ewp_bind [AppLCtx _]); first done.
-    iApply ewp_ms_prot_mono; [iApply sig_le_nil|]. 
     iApply (ewp_mono with "[HΓ₂]"); first (by iApply "He₁").
-    iIntros "% [Hτκ HΓ₃] !> /=".
-    iApply ewp_ms_prot_mono; [iApply sig_le_nil|]. 
+    iIntros "% [Hτκ HΓ₃'] !> /=".
     iApply (ewp_mono with "[Hτ Hτκ]"); first (by iApply "Hτκ").
     iIntros "% $ !> //=".
   Qed.
 
-  Lemma sem_typed_seq Γ₁ Γ₂ Γ₃ e₁ e₂ τ ρs κ: 
-    Γ₁ ⊨ e₁ : ρs : τ ⊨ Γ₂ -∗
-    Γ₂ ⊨ e₂ : ρs : κ ⊨ Γ₃ -∗
-    Γ₁ ⊨ (e₁ ;; e₂) : ρs : κ ⊨ Γ₃.
+  Lemma sem_typed_seq Γ₁ Γ₂ Γ₃ e₁ e₂ τ σ κ: 
+    Γ₁ ⊨ e₁ : σ : τ ⊨ Γ₂ -∗
+    Γ₂ ⊨ e₂ : σ : κ ⊨ Γ₃ -∗
+    Γ₁ ⊨ (e₁ ;; e₂) : σ : κ ⊨ Γ₃.
   Proof.
     iIntros "#He₁ #He₂ !# %vs HΓ₁ /=".
     iApply (ewp_bind ([AppRCtx _])); first done. simpl.
@@ -454,46 +400,29 @@ Section compatibility.
     iIntros "!# % [Hτκ HΓ₃] !> /=". iFrame.
   Qed.
 
-  Lemma sem_typed_pair Γ₁ Γ₂ Γ₃ e₁ e₂ τ ρs κ: 
-    Γ₂ ⊨ e₁ : ⟨ρs.1,⟩ : τ ⊨ Γ₃ -∗
-    Γ₁ ⊨ e₂ : ρs : κ ⊨ Γ₂ -∗
-    Γ₁ ⊨ (e₁,e₂) : ρs : (τ × κ) ⊨ Γ₃.
+  Lemma sem_typed_pair Γ₁ Γ₂ Γ₃ e₁ e₂ τ σ κ: 
+    Γ₂ ⊨ e₁ : σ : τ ⊨ Γ₃ -∗
+    Γ₁ ⊨ e₂ : σ : κ ⊨ Γ₂ -∗
+    Γ₁ ⊨ (e₁,e₂) : σ : (τ × κ) ⊨ Γ₃.
   Proof.
     iIntros "#He₁ #He₂ !# %vs HΓ₁ //=".
     iApply (ewp_bind ([PairRCtx (subst_map vs e₁)])); first done.
-    iApply (ewp_pers_mono with "[HΓ₁]"); first (by iApply "He₂").
-    iIntros "!# % [Hτ HΓ₂] !> /=".
+    iApply (ewp_mono with "[HΓ₁]"); first (by iApply "He₂").
+    iIntros "% [Hτ HΓ₂] !> /=".
     iApply (ewp_bind ([PairLCtx v])); first done.
-    iApply ewp_ms_prot_mono; [iApply sig_le_nil|].
     iApply (ewp_mono with "[HΓ₂]"); first (by iApply "He₁").
     iIntros (w) "[Hκw HΓ₃] //= !>". ewp_pure_steps.
     solve_env.
   Qed.
   
-  Lemma sem_typed_pair_ms Γ₁ Γ₂ Γ₃ (x₁ x₂ : string) e₁ e₂ τ ρs κ: 
-    x₂ ∉ env_dom Γ₂ → x₂ ∉ env_dom Γ₃ → x₁ ∉ env_dom Γ₃ → x₁ ≠ x₂ →
-    copy_ty κ -∗
-    Γ₂ ⊨ e₁ : ρs : τ ⊨ Γ₃ -∗
-    Γ₁ ⊨ e₂ : ρs : κ ⊨ Γ₂ -∗
-    Γ₁ ⊨ (let: x₂ := e₂ in let: x₁ := e₁ in (x₁,x₂)) : ρs : (τ × κ) ⊨ Γ₃.
-  Proof.
-    iIntros (????) "#Hcpy #He₁ #He₂".
-    iApply (sem_typed_let _ Γ₂); solve_sidecond.
-    iApply (sem_typed_let _ ((x₂, κ) :: Γ₃)); solve_sidecond.
-    { iApply sem_typed_frame_ms; first done. iApply "He₁". }
-    iApply sem_typed_sub_nil.
-    iApply (sem_typed_pair _ ((x₁, τ) :: Γ₃)); [iApply sem_typed_var|].
-    iApply sem_typed_swap_second.
-    iApply sem_typed_var.
-  Qed.
 
-  Lemma sem_typed_pair_elim Γ₁ Γ₂ Γ₃ x₁ x₂ e₁ e₂ τ ρs κ ι: 
+  Lemma sem_typed_pair_elim Γ₁ Γ₂ Γ₃ x₁ x₂ e₁ e₂ τ σ κ ι: 
     x₁ ∉ (env_dom Γ₂) → x₂ ∉ (env_dom Γ₂) →
     x₁ ∉ (env_dom Γ₃) → x₂ ∉ (env_dom Γ₃) →
     x₁ ≠ x₂ →
-    Γ₁ ⊨ e₁ : ρs : (τ × κ) ⊨ Γ₂ -∗
-    (x₁, τ) :: (x₂, κ) :: Γ₂ ⊨ e₂ : ρs : ι ⊨ Γ₃ -∗
-    Γ₁ ⊨ (let: (x₁, x₂) := e₁ in e₂) : ρs : ι ⊨ Γ₃.
+    Γ₁ ⊨ e₁ : σ : (τ × κ) ⊨ Γ₂ -∗
+    (x₁, τ) :: (x₂, κ) :: Γ₂ ⊨ e₂ : σ : ι ⊨ Γ₃ -∗
+    Γ₁ ⊨ (let: (x₁, x₂) := e₁ in e₂) : σ : ι ⊨ Γ₃.
   Proof.
     iIntros (?????) "#He₁ #He₂ !# %vs HΓ₁ //=". ewp_pure_steps.
     set ex1x2 := (λ: x₁ x₂, subst_map (binder_delete x₂ 
@@ -517,9 +446,9 @@ Section compatibility.
       by rewrite -(env_sem_typed_insert _ _ x₁ v₁).
   Qed.
   
-  Lemma sem_typed_left_inj Γ₁ Γ₂ e τ ρs κ: 
-    Γ₁ ⊨ e : ρs : τ ⊨ Γ₂ -∗
-    Γ₁ ⊨ InjL e : ρs : (τ + κ) ⊨ Γ₂.
+  Lemma sem_typed_left_inj Γ₁ Γ₂ e τ σ κ: 
+    Γ₁ ⊨ e : σ : τ ⊨ Γ₂ -∗
+    Γ₁ ⊨ InjL e : σ : (τ + κ) ⊨ Γ₂.
   Proof.
     iIntros "#He !# %vs HΓ₁ //=".
     iApply (ewp_bind [InjLCtx]); first done.
@@ -528,9 +457,9 @@ Section compatibility.
     iFrame. iExists v. iLeft. by iFrame.
   Qed.
 
-  Lemma sem_typed_right_inj Γ₁ Γ₂ e τ ρs κ: 
-    Γ₁ ⊨ e : ρs : κ ⊨ Γ₂ -∗
-    Γ₁ ⊨ InjR e : ρs : (τ + κ) ⊨ Γ₂.
+  Lemma sem_typed_right_inj Γ₁ Γ₂ e τ σ κ: 
+    Γ₁ ⊨ e : σ : κ ⊨ Γ₂ -∗
+    Γ₁ ⊨ InjR e : σ : (τ + κ) ⊨ Γ₂.
   Proof.
     iIntros "#He !# %vs HΓ₁ //=".
     iApply (ewp_bind [InjRCtx]); first done.
@@ -539,12 +468,12 @@ Section compatibility.
     iFrame. iExists v. iRight. by iFrame.
   Qed.
 
-  Lemma sem_typed_match Γ₁ Γ₂ Γ₃ e₁ x y e₂ e₃ τ ρs κ ι: 
+  Lemma sem_typed_match Γ₁ Γ₂ Γ₃ e₁ x y e₂ e₃ τ σ κ ι: 
     x ∉ env_dom Γ₂ → x ∉ env_dom Γ₃ → y ∉ env_dom Γ₂ → y ∉ env_dom Γ₃ →
-    Γ₁ ⊨ e₁ : ρs : (τ + κ) ⊨ Γ₂ -∗
-    (x, τ) ::? Γ₂ ⊨ e₂ : ρs : ι ⊨ Γ₃ -∗
-    (y, κ) ::? Γ₂ ⊨ e₃ : ρs : ι ⊨ Γ₃ -∗
-    Γ₁ ⊨ match: e₁ with InjL x => e₂ | InjR y => e₃ end : ρs : ι ⊨ Γ₃.
+    Γ₁ ⊨ e₁ : σ : (τ + κ) ⊨ Γ₂ -∗
+    (x, τ) ::? Γ₂ ⊨ e₂ : σ : ι ⊨ Γ₃ -∗
+    (y, κ) ::? Γ₂ ⊨ e₃ : σ : ι ⊨ Γ₃ -∗
+    Γ₁ ⊨ match: e₁ with InjL x => e₂ | InjR y => e₃ end : σ : ι ⊨ Γ₃.
   Proof.
     iIntros (????) "#He₁ #He₂ #He₃ !# %vs HΓ₁ //=".
     iApply (ewp_bind [CaseCtx _ _]); first done.
@@ -563,24 +492,24 @@ Section compatibility.
   Qed.
 
   Lemma sem_typed_none Γ₁ τ: 
-    ⊢ Γ₁ ⊨ NONE : ⟨⟩ : Option τ ⊨ Γ₁.
+    ⊢ Γ₁ ⊨ NONE : ⊥ : Option τ ⊨ Γ₁.
   Proof.
     iIntros. iApply sem_typed_left_inj. iApply sem_typed_unit. 
   Qed.
 
-  Lemma sem_typed_some Γ₁ Γ₂ e ρs τ: 
-    Γ₁ ⊨ e : ρs : τ ⊨ Γ₂ -∗ 
-    Γ₁ ⊨ SOME e : ρs : Option τ ⊨ Γ₂.
+  Lemma sem_typed_some Γ₁ Γ₂ e σ τ: 
+    Γ₁ ⊨ e : σ : τ ⊨ Γ₂ -∗ 
+    Γ₁ ⊨ SOME e : σ : Option τ ⊨ Γ₂.
   Proof.
     iIntros "He". iApply sem_typed_right_inj. iApply "He".
   Qed.
 
-  Lemma sem_typed_match_option Γ₁ Γ₂ Γ₃ e₁ x e₂ e₃ ρs κ ι: 
+  Lemma sem_typed_match_option Γ₁ Γ₂ Γ₃ e₁ x e₂ e₃ σ κ ι: 
     x ∉ env_dom Γ₂ → x ∉ env_dom Γ₃ →
-    Γ₁ ⊨ e₁ : ρs : Option κ ⊨ Γ₂ -∗
-    Γ₂ ⊨ e₂ : ρs : ι ⊨ Γ₃ -∗
-    (x, κ) :: Γ₂ ⊨ e₃ : ρs : ι ⊨ Γ₃ -∗
-    Γ₁ ⊨ match: e₁ with NONE => e₂ | SOME x => e₃ end : ρs : ι ⊨ Γ₃.
+    Γ₁ ⊨ e₁ : σ : Option κ ⊨ Γ₂ -∗
+    Γ₂ ⊨ e₂ : σ : ι ⊨ Γ₃ -∗
+    (x, κ) :: Γ₂ ⊨ e₃ : σ : ι ⊨ Γ₃ -∗
+    Γ₁ ⊨ match: e₁ with NONE => e₂ | SOME x => e₃ end : σ : ι ⊨ Γ₃.
   Proof.
     iIntros (??) "#He₁ #He₂ #He₃ !# %vs HΓ₁ //=".
     iApply (ewp_bind [CaseCtx _ _]); first done.
@@ -592,36 +521,30 @@ Section compatibility.
       iIntros "!# % [$ HΓ₃] //=". solve_env.
   Qed.
 
-  Lemma bin_op_copy_types τ κ ι op :
-    typed_bin_op op τ κ ι → ⊢ copy_ty τ ∗ copy_ty κ ∗ copy_ty ι.
-  Proof. intros []; (iSplit; [|iSplit]); solve_copy. Qed.
-
-  Lemma sem_typed_bin_op Γ₁ Γ₂ Γ₃ e₁ e₂ op τ κ ι ρs: 
+  Lemma sem_typed_bin_op Γ₁ Γ₂ Γ₃ e₁ e₂ op τ κ ι σ: 
     typed_bin_op op τ κ ι →
-    Γ₂ ⊨ e₁ : ρs : τ ⊨ Γ₃ -∗
-    Γ₁ ⊨ e₂ : ρs : κ ⊨ Γ₂ -∗
-    Γ₁ ⊨ BinOp op e₁ e₂ : ρs : ι ⊨ Γ₃.
+    Γ₂ ⊨ e₁ : σ : τ ⊨ Γ₃ -∗
+    Γ₁ ⊨ e₂ : σ : κ ⊨ Γ₂ -∗
+    Γ₁ ⊨ BinOp op e₁ e₂ : σ : ι ⊨ Γ₃.
   Proof.
     iIntros (Hop) "#He₁ #He₂ !# %vs HΓ₁ //=".
-    iDestruct (bin_op_copy_types _ _ _ _ Hop) as "[Hcpyτ [Hcpyκ Hcpyι]]". 
     iApply (ewp_bind [BinOpRCtx _ _]); first done.
-    iApply (ewp_pers_mono with "[HΓ₁]"); [iApply "He₂"; solve_env|eauto].
-    iIntros "!# %v [Hκ HΓ₂] //= !>". 
+    iApply (ewp_mono with "[HΓ₁]"); [iApply "He₂"; solve_env|eauto].
+    iIntros "%v [Hκ HΓ₂] //= !>". 
     iApply (ewp_bind [BinOpLCtx _ _]); first done.
-    iApply (ewp_pers_mono with "[HΓ₂]"); [iApply "He₁"; solve_env|eauto].
-    iDestruct ("Hcpyκ" with "Hκ") as "#Hκ'".
-    iIntros "!# %w [Hτ HΓ₂] //= !>".
+    iApply (ewp_mono with "[HΓ₂]"); [iApply "He₁"; solve_env|eauto].
+    iIntros "%w [Hτ HΓ₂] //= !>".
     destruct op; inversion_clear Hop;
       iDestruct "Hτ" as "(%n1 & ->)";
-      iDestruct "Hκ'" as "(%n2 & ->)";
+      iDestruct "Hκ" as "(%n2 & ->)";
       ewp_pure_steps; try done; eauto.
   Qed.
   
-  Lemma sem_typed_if Γ₁ Γ₂ Γ₃ e₁ e₂ e₃ ρs τ: 
-    Γ₁ ⊨ e₁ : ρs : 𝔹 ⊨ Γ₂ -∗
-    Γ₂ ⊨ e₂ : ρs : τ ⊨ Γ₃ -∗
-    Γ₂ ⊨ e₃ : ρs : τ ⊨ Γ₃ -∗
-    Γ₁ ⊨ (if: e₁ then e₂ else e₃) : ρs : τ ⊨ Γ₃.
+  Lemma sem_typed_if Γ₁ Γ₂ Γ₃ e₁ e₂ e₃ σ τ: 
+    Γ₁ ⊨ e₁ : σ : 𝔹 ⊨ Γ₂ -∗
+    Γ₂ ⊨ e₂ : σ : τ ⊨ Γ₃ -∗
+    Γ₂ ⊨ e₃ : σ : τ ⊨ Γ₃ -∗
+    Γ₁ ⊨ (if: e₁ then e₂ else e₃) : σ : τ ⊨ Γ₃.
   Proof.
     iIntros "#He₁ #He₂ #He₃ !# %vs HΓ₁ //=".
     iApply (ewp_bind [IfCtx (subst_map vs e₂) (subst_map vs e₃)]) ;first done.
@@ -633,10 +556,10 @@ Section compatibility.
   Qed.
   
   (* Type abstraction and application *)
-  Lemma sem_typed_TLam Γ₁ Γ₂ ρs e C : 
+  Lemma sem_typed_TLam Γ₁ Γ₂ e C : 
     copy_env Γ₁ -∗
-    (∀ α, Γ₁ ⊨ e : ρs : C α ⊨ []) -∗
-    Γ₁ ++ Γ₂ ⊨ (Λ: e) : ⟨⟩ : (∀T: α , ρs , C α)%T ⊨ Γ₂.
+    (∀ α, Γ₁ ⊨ e : ⊥ : C α ⊨ []) -∗
+    Γ₁ ++ Γ₂ ⊨ (Λ: e) : ⊥ : (∀T: α , C α)%T ⊨ Γ₂.
   Proof.
     iIntros "#Hcpy #He !# %vs HΓ₁₂ //=".
     iDestruct (env_sem_typed_app with "HΓ₁₂") as "[HΓ₁ HΓ₂]".
@@ -646,66 +569,52 @@ Section compatibility.
     iIntros "!# %w [$ _] //=".
   Qed.
 
-  Lemma sem_typed_TApp Γ₁ Γ₂ e ρs τ C :
-    copy_env Γ₂ -∗
-    Γ₁ ⊨ e : ρs : (∀T: α , ρs , C α) ⊨ Γ₂ -∗
-    Γ₁ ⊨ e <_> : ρs : C τ ⊨ Γ₂. 
+  Lemma sem_typed_TApp Γ₁ Γ₂ e σ τ C :
+    Γ₁ ⊨ e : σ : (∀T: α , C α) ⊨ Γ₂ -∗
+    Γ₁ ⊨ e <_> : σ : C τ ⊨ Γ₂. 
   Proof.
-    iIntros "#Hcpy #He !# %vs HΓ₁ /=".
+    iIntros "#He !# %vs HΓ₁ /=".
     iApply (ewp_bind [AppLCtx _]); first done.
-    iApply (ewp_pers_mono with "[HΓ₁]"); [iApply "He"; solve_env|].
-    iIntros "!# %w [Hw HΓ₂] //= !>".
-    iApply (ewp_pers_mono with "[Hw]"); [iApply "Hw"|].
-    iDestruct ("Hcpy" with "HΓ₂") as "#HΓ₂'".
-    iIntros "!# % HC !>". iFrame "#∗".
-  Qed.
-
-  Lemma sem_typed_TApp_os Γ₁ Γ₂ (x : string) e ρ τ C :
-    x ∉ env_dom Γ₂ → 
-    Γ₁ ⊨ e : ⟨ρ,⟩ : (∀T: α , ⟨ρ,⟩ , C α) ⊨ Γ₂ -∗
-    Γ₁ ⊨ (let: x := e in x <_>) : ⟨ρ,⟩ : C τ ⊨ Γ₂. 
-  Proof.
-    iIntros (?) "#He". 
-    iApply (sem_typed_let _ Γ₂); solve_sidecond.
-    iApply sem_typed_swap_env_singl. rewrite - {3} (app_nil_r Γ₂).
-    iApply sem_typed_frame_env_os. iApply sem_typed_TApp; solve_copy.
-    iApply sem_typed_sub_nil. iApply sem_typed_var.
+    iApply (ewp_mono with "[HΓ₁]"); [iApply "He"; solve_env|].
+    iIntros "%w [Hw HΓ₂] //= !>".
+    iApply ewp_os_prot_mono; [iApply sig_le_nil|].
+    iApply (ewp_mono with "[Hw]"); [iApply "Hw"|].
+    iIntros "% HC !>". iFrame "#∗".
   Qed.
 
   (* Signature abstraction and application *)
   Lemma sem_typed_SLam Γ₁ Γ₂ e C : 
     copy_env Γ₁ -∗
-    (∀ θ, Γ₁ ⊨ e : ⟨⟩ : C θ ⊨ []) -∗
-    Γ₁ ++ Γ₂ ⊨ (Λ: e) : ⟨⟩ : (∀R: θ , C θ)%T ⊨ Γ₂.
+    (∀ θ, Γ₁ ⊨ e : ⊥ : C θ ⊨ []) -∗
+    Γ₁ ++ Γ₂ ⊨ (Λ: e) : ⊥ : (∀S: θ , C θ)%T ⊨ Γ₂.
   Proof.
     iIntros "#Hcpy #He !# %vs HΓ₁₂ /=".
     iDestruct (env_sem_typed_app with "HΓ₁₂") as "[HΓ₁ HΓ₂]".
     ewp_pure_steps. iFrame.
     iDestruct ("Hcpy" with "HΓ₁") as "#HΓ₁'".
-    iIntros (ρs). ewp_pure_steps. iIntros "!#".
+    iIntros (σ). ewp_pure_steps. iIntros "!#".
     ewp_pure_steps.
     iApply ewp_pers_mono; [by iApply "He"|].
     iIntros "!# % [$ _] //=".
   Qed.
 
-  Lemma sem_typed_SApp Γ₁ Γ₂ e ρs ρs' C : 
-    Γ₁ ⊨ e : ρs : (∀R: θ , C θ) ⊨ Γ₂ -∗
-    Γ₁ ⊨ e <_> : ρs : C ρs' ⊨ Γ₂. 
+  Lemma sem_typed_SApp Γ₁ Γ₂ e σ σ' C : 
+    Γ₁ ⊨ e : σ : (∀S: θ , C θ) ⊨ Γ₂ -∗
+    Γ₁ ⊨ e <_> : σ : C σ' ⊨ Γ₂. 
   Proof.
     iIntros "#He !# %vs HΓ₁ /=".
     iApply (ewp_bind [AppLCtx _]); first done.
     iApply (ewp_pers_mono with "[HΓ₁]"); [by iApply "He"|].
     iIntros "!# %v [HC HΓ₂] /= !>".
     iApply ewp_os_prot_mono; [iApply sig_le_nil|].
-    iApply ewp_ms_prot_mono; [iApply sig_le_nil|].
-    iApply (ewp_mono with "[HC]"); [iApply ("HC" $! ρs')|].
-    iIntros "%w HCρ !>". iFrame "∗#".
+    iApply (ewp_mono with "[HC]"); [iApply ("HC" $! σ')|].
+    iIntros "%w HCσ !>". iFrame "∗#".
   Qed.
 
   (* Existential type packing and unpacking *)
-  Lemma sem_typed_pack Γ₁ Γ₂ ρs e C τ :
-    Γ₁ ⊨ e : ρs : C τ ⊨ Γ₂ -∗
-    Γ₁ ⊨ (pack: e) : ρs : (∃: α, C α) ⊨ Γ₂. 
+  Lemma sem_typed_pack Γ₁ Γ₂ σ e C τ :
+    Γ₁ ⊨ e : σ : C τ ⊨ Γ₂ -∗
+    Γ₁ ⊨ (pack: e) : σ : (∃: α, C α) ⊨ Γ₂. 
   Proof.
     iIntros "#He %vs !# HΓ₁ //=".
     iApply (ewp_bind [AppRCtx _]); first done.
@@ -715,11 +624,11 @@ Section compatibility.
     by iExists τ. 
   Qed.
 
-  Lemma sem_typed_unpack Γ₁ Γ₂ Γ₃ x ρs e₁ e₂ κ C :
+  Lemma sem_typed_unpack Γ₁ Γ₂ Γ₃ x σ e₁ e₂ κ C :
     x ∉ env_dom Γ₂ → x ∉ env_dom Γ₃ →
-    Γ₁ ⊨ e₁ : ρs : (∃: α, C α) ⊨ Γ₂ -∗
-    (∀ τ, (x, C τ) :: Γ₂ ⊨ e₂ : ρs : κ ⊨ Γ₃) -∗
-    Γ₁ ⊨ (unpack: x := e₁ in e₂) : ρs : κ ⊨ Γ₃.
+    Γ₁ ⊨ e₁ : σ : (∃: α, C α) ⊨ Γ₂ -∗
+    (∀ τ, (x, C τ) :: Γ₂ ⊨ e₂ : σ : κ ⊨ Γ₃) -∗
+    Γ₁ ⊨ (unpack: x := e₁ in e₂) : σ : κ ⊨ Γ₃.
   Proof.
     iIntros (??) "#He₁ #He₂ %vs !# HΓ₁ //=".
     iApply (ewp_bind [AppRCtx _]); first done.
@@ -731,9 +640,9 @@ Section compatibility.
   Qed.
 
   (* Recursive type rules *)
-  Lemma sem_typed_fold Γ₁ Γ₂ e ρs C `{NonExpansive C}:
-    Γ₁ ⊨ e : ρs : (C (μT: α, C α)) ⊨ Γ₂ -∗
-    Γ₁ ⊨ (fold: e) : ρs : (μT: α, C α) ⊨ Γ₂.
+  Lemma sem_typed_fold Γ₁ Γ₂ e σ C `{NonExpansive C}:
+    Γ₁ ⊨ e : σ : (C (μT: α, C α)) ⊨ Γ₂ -∗
+    Γ₁ ⊨ (fold: e) : σ : (μT: α, C α) ⊨ Γ₂.
   Proof.
     iIntros "#He %vs !# HΓ₁ //=".
     iApply (ewp_bind [AppRCtx _]); first done.
@@ -743,9 +652,9 @@ Section compatibility.
     iFrame. by iApply sem_ty_rec_unfold. 
   Qed.
 
-  Lemma sem_typed_unfold Γ₁ Γ₂ e ρs C `{NonExpansive C}:
-    Γ₁ ⊨ e : ρs : (μT: α, C α) ⊨ Γ₂ -∗
-    Γ₁ ⊨ (unfold: e) : ρs : (C (μT: α, C α)) ⊨ Γ₂.
+  Lemma sem_typed_unfold Γ₁ Γ₂ e σ C `{NonExpansive C}:
+    Γ₁ ⊨ e : σ : (μT: α, C α) ⊨ Γ₂ -∗
+    Γ₁ ⊨ (unfold: e) : σ : (C (μT: α, C α)) ⊨ Γ₂.
   Proof.
     iIntros "#He %vs !# HΓ₁ //=".
     iApply (ewp_bind [AppRCtx _]); first done. 
@@ -758,7 +667,7 @@ Section compatibility.
 
   (* List type rules *)
   Lemma sem_typed_nil Γ τ: 
-    ⊢ Γ ⊨ NIL : ⟨⟩ : List τ ⊨ Γ.
+    ⊢ Γ ⊨ NIL : ⊥ : List τ ⊨ Γ.
   Proof.
     iIntros "!# %vs HΓ //=". 
     ewp_pure_steps. unfold sem_ty_list. 
@@ -766,17 +675,16 @@ Section compatibility.
     unfold ListF. iExists #(). by iLeft.
   Qed.
   
-  Lemma sem_typed_cons Γ₁ Γ₂ Γ₃ e₁ e₂ ρs τ:
-    Γ₂ ⊨ e₁ : ⟨ρs.1,⟩ : τ ⊨ Γ₃-∗
-    Γ₁ ⊨ e₂ : ρs : List τ ⊨ Γ₂-∗
-    Γ₁ ⊨ CONS e₁ e₂ : ρs : List τ ⊨ Γ₃.
+  Lemma sem_typed_cons Γ₁ Γ₂ Γ₃ e₁ e₂ σ τ:
+    Γ₂ ⊨ e₁ : σ : τ ⊨ Γ₃-∗
+    Γ₁ ⊨ e₂ : σ : List τ ⊨ Γ₂-∗
+    Γ₁ ⊨ CONS e₁ e₂ : σ : List τ ⊨ Γ₃.
   Proof.
     iIntros "#He₁ #He₂ !# %vs HΓ₁ //=". 
     iApply (ewp_bind [InjRCtx; PairRCtx _]); first done.
-    iApply (ewp_pers_mono with "[HΓ₁]"); [by iApply "He₂"|].
-    iIntros "!# %l [Hl HΓ₂] //= !>".
+    iApply (ewp_mono with "[HΓ₁]"); [by iApply "He₂"|].
+    iIntros "%l [Hl HΓ₂] //= !>".
     iApply (ewp_bind [InjRCtx; PairLCtx _]); first done.
-    iApply ewp_ms_prot_mono; [iApply sig_le_nil|].
     iApply (ewp_mono with "[HΓ₂]"); [by iApply "He₁"|].
     iIntros "%x [Hx HΓ₃] //= !>". ewp_pure_steps.
     unfold sem_ty_list. rewrite !sem_ty_rec_unfold.
@@ -785,34 +693,17 @@ Section compatibility.
     by rewrite sem_ty_rec_unfold. 
   Qed.
 
-  Lemma sem_typed_cons_ms Γ₁ Γ₂ Γ₃ (x₁ x₂ : string) e₁ e₂ ρs τ:
-    x₂ ∉ env_dom Γ₂ → x₂ ∉ env_dom Γ₃ → x₁ ∉ env_dom Γ₃ → x₁ ≠ x₂ → 
-    copy_ty τ -∗
-    Γ₂ ⊨ e₁ : ρs : τ ⊨ Γ₃ -∗
-    Γ₁ ⊨ e₂ : ρs : List τ ⊨ Γ₂-∗
-    Γ₁ ⊨ (let: x₂ := e₂ in let: x₁ := e₁ in CONS x₁ x₂) : ρs : List τ ⊨ Γ₃.
-  Proof.
-    iIntros (????) "#Hcpy #He₁ #He₂".
-    iApply (sem_typed_let _ Γ₂); solve_sidecond.
-    iApply (sem_typed_let _ ((x₂, List τ) :: Γ₃)); solve_sidecond.
-    { iApply sem_typed_frame_ms; first by iApply copy_ty_list. iApply "He₁". }
-    iApply sem_typed_sub_nil.
-    iApply (sem_typed_cons _ ((x₁, τ) :: Γ₃)); [iApply sem_typed_var|].
-    iApply sem_typed_swap_second.
-    iApply sem_typed_var.
-  Qed.
-
-  Lemma sem_typed_match_list Γ₁ Γ₂ Γ₃ x xs e₁ e₂ e₃ ρs τ κ :
+  Lemma sem_typed_match_list Γ₁ Γ₂ Γ₃ x xs e₁ e₂ e₃ σ τ κ :
     x ∉ (env_dom Γ₂) -> xs ∉ (env_dom Γ₂) ->
     x ∉ (env_dom Γ₃) -> xs ∉ (env_dom Γ₃) ->
     x ≠ xs ->
-    Γ₁ ⊨ e₁ : ρs : List τ ⊨ Γ₂ -∗
-    Γ₂ ⊨ e₂ : ρs : κ ⊨ Γ₃ -∗
-    (x, τ) :: (xs, List τ) :: Γ₂ ⊨ e₃ : ρs : κ ⊨ Γ₃ -∗
+    Γ₁ ⊨ e₁ : σ : List τ ⊨ Γ₂ -∗
+    Γ₂ ⊨ e₂ : σ : κ ⊨ Γ₃ -∗
+    (x, τ) :: (xs, List τ) :: Γ₂ ⊨ e₃ : σ : κ ⊨ Γ₃ -∗
     Γ₁ ⊨ list-match: e₁ with 
             CONS x => xs => e₃ 
           | NIL => e₂
-         end : ρs : κ ⊨ Γ₃.
+         end : σ : κ ⊨ Γ₃.
   Proof.
     iIntros (?????) "#He₁ #He₂ #He₃ !# %vs HΓ₁ //=".
     iApply (ewp_bind [CaseCtx _ _]); first done. simpl.
@@ -841,9 +732,9 @@ Section compatibility.
 
   (* Reference rules *)
   
-  Lemma sem_typed_alloc Γ₁ Γ₂ e ρs τ: 
-    Γ₁ ⊨ e : ρs : τ ⊨ Γ₂ -∗
-    Γ₁ ⊨ ref e : ρs : Ref τ ⊨ Γ₂.
+  Lemma sem_typed_alloc Γ₁ Γ₂ e σ τ: 
+    Γ₁ ⊨ e : σ : τ ⊨ Γ₂ -∗
+    Γ₁ ⊨ ref e : σ : Ref τ ⊨ Γ₂.
   Proof.
     iIntros "#He !# %vs HΓ₁ //=".
     iApply (ewp_bind [AllocCtx]); first done. simpl.
@@ -853,7 +744,7 @@ Section compatibility.
   Qed.
   
   Lemma sem_typed_load Γ x τ: 
-    ⊢ ((x, Ref τ) :: Γ ⊨ !x : ⟨⟩ : τ ⊨ (x, Ref Moved) :: Γ).
+    ⊢ ((x, Ref τ) :: Γ ⊨ !x : ⊥ : τ ⊨ (x, Ref Moved) :: Γ).
   Proof.
     iIntros "%vs !# //= [%v (%Hrw & (%w & -> & (%l & Hl & Hτ)) & HΓ)]".
     rewrite Hrw. iApply (ewp_load with "Hl").
@@ -862,7 +753,7 @@ Section compatibility.
   
   Lemma sem_typed_load_copy Γ x τ: 
     copy_ty τ -∗
-    ((x, Ref τ) :: Γ ⊨ !x : ⟨⟩ : τ ⊨ (x, Ref τ) :: Γ).
+    ((x, Ref τ) :: Γ ⊨ !x : ⊥ : τ ⊨ (x, Ref τ) :: Γ).
   Proof.
     iIntros "#Hcpy %vs !# //= [%v (%Hrw & (%w & -> & (%l & Hl & Hτ)) & HΓ)]".
     rewrite Hrw. iApply (ewp_load with "Hl").
@@ -870,9 +761,9 @@ Section compatibility.
     iIntros "!> Hl !>". solve_env.
   Qed.
 
-  Lemma sem_typed_store Γ₁ Γ₂ x e ρs τ κ ι: 
-    (x, Ref τ) :: Γ₁ ⊨ e : ρs : ι ⊨ (x, Ref κ) :: Γ₂ -∗
-    (x, Ref τ) :: Γ₁ ⊨ (x <- e) : ρs : () ⊨ (x, Ref ι) :: Γ₂.
+  Lemma sem_typed_store Γ₁ Γ₂ x e σ τ κ ι: 
+    (x, Ref τ) :: Γ₁ ⊨ e : σ : ι ⊨ (x, Ref κ) :: Γ₂ -∗
+    (x, Ref τ) :: Γ₁ ⊨ (x <- e) : σ : () ⊨ (x, Ref ι) :: Γ₂.
   Proof.
     iIntros "#He !# %vs //= HΓ₁' //=".
     iApply (ewp_bind [StoreRCtx _]); first done. simpl.
@@ -882,9 +773,9 @@ Section compatibility.
     iIntros "!> !> Hl !>". solve_env. 
   Qed.
 
-  Lemma sem_typed_alloc_cpy Γ₁ Γ₂ e ρs τ: 
-    Γ₁ ⊨ e : ρs : τ ⊨ Γ₂ -∗
-    Γ₁ ⊨ ref e : ρs : Refᶜ  τ ⊨ Γ₂.
+  Lemma sem_typed_alloc_cpy Γ₁ Γ₂ e σ τ: 
+    Γ₁ ⊨ e : σ : τ ⊨ Γ₂ -∗
+    Γ₁ ⊨ ref e : σ : Refᶜ  τ ⊨ Γ₂.
   Proof.
     iIntros "#He !# %vs HΓ₁ //=".
     iApply (ewp_bind [AllocCtx]); first done. simpl.
@@ -897,10 +788,10 @@ Section compatibility.
     iModIntro. iExists l. by auto.
   Qed.
 
-  Lemma sem_typed_load_cpy Γ₁ Γ₂ e ρs τ: 
+  Lemma sem_typed_load_cpy Γ₁ Γ₂ e σ τ: 
     copy_ty τ -∗
-    Γ₁ ⊨ e : ρs : Refᶜ τ ⊨ Γ₂ -∗
-    Γ₁ ⊨ !e : ρs : τ ⊨ Γ₂.
+    Γ₁ ⊨ e : σ : Refᶜ τ ⊨ Γ₂ -∗
+    Γ₁ ⊨ !e : σ : τ ⊨ Γ₂.
   Proof.
     iIntros "#Hcpy #He %vs !# //= HΓ₁".
     iApply (ewp_bind [LoadCtx]); first done.
@@ -914,17 +805,16 @@ Section compatibility.
     iMod ("Hclose" with "[Hl]"); solve_env.
   Qed.
 
-  Lemma sem_typed_store_cpy Γ₁ Γ₂ Γ₃ e₁ e₂ ρs τ: 
-    Γ₂ ⊨ e₁ : ⟨ρs.1,⟩ : Refᶜ τ ⊨ Γ₃ -∗
-    Γ₁ ⊨ e₂ : ρs : τ ⊨ Γ₂ -∗
-    Γ₁ ⊨ (e₁ <- e₂) : ρs : () ⊨ Γ₃.
+  Lemma sem_typed_store_cpy Γ₁ Γ₂ Γ₃ e₁ e₂ σ τ: 
+    Γ₂ ⊨ e₁ : σ : Refᶜ τ ⊨ Γ₃ -∗
+    Γ₁ ⊨ e₂ : σ : τ ⊨ Γ₂ -∗
+    Γ₁ ⊨ (e₁ <- e₂) : σ : () ⊨ Γ₃.
   Proof.
     iIntros "#He₁ #He₂ %vs !# /= HΓ₁ /=".
     iApply (ewp_bind [StoreRCtx _]); first done. simpl.
-    iApply (ewp_pers_mono with "[HΓ₁]"); [by iApply "He₂"|].
-    iIntros "!# %w [Hτ HΓ₂] !>". 
+    iApply (ewp_mono with "[HΓ₁]"); [by iApply "He₂"|].
+    iIntros "%w [Hτ HΓ₂] !>". 
     iApply (ewp_bind [StoreLCtx _]); first done. simpl.
-    iApply ewp_ms_prot_mono; [iApply sig_le_nil|].
     iApply (ewp_mono with "[HΓ₂]"); [by iApply "He₁"|].
     iIntros "%u [(%l & -> & Hinv) HΓ₃] !>".
     iApply (ewp_atomic _ (⊤ ∖ ↑tyN.@l)).
@@ -934,17 +824,16 @@ Section compatibility.
     iMod ("Hclose" with "[Hl Hτ]"); solve_env.
   Qed.
 
-  Lemma sem_typed_replace_cpy Γ₁ Γ₂ Γ₃ e₁ e₂ ρs τ: 
-    Γ₂ ⊨ e₁ : ⟨ρs.1,⟩ : Refᶜ τ ⊨ Γ₃ -∗
-    Γ₁ ⊨ e₂ : ρs : τ ⊨ Γ₂ -∗
-    Γ₁ ⊨ (e₁ <!- e₂) : ρs : τ ⊨ Γ₃.
+  Lemma sem_typed_replace_cpy Γ₁ Γ₂ Γ₃ e₁ e₂ σ τ: 
+    Γ₂ ⊨ e₁ : σ : Refᶜ τ ⊨ Γ₃ -∗
+    Γ₁ ⊨ e₂ : σ : τ ⊨ Γ₂ -∗
+    Γ₁ ⊨ (e₁ <!- e₂) : σ : τ ⊨ Γ₃.
   Proof.
     iIntros "#He₁ #He₂ %vs !# /= HΓ₁ /=".
     iApply (ewp_bind [ReplaceRCtx _]); first done. simpl.
-    iApply (ewp_pers_mono with "[HΓ₁]"); [by iApply "He₂"|].
-    iIntros "!# %w [Hτ HΓ₂] !>". 
+    iApply (ewp_mono with "[HΓ₁]"); [by iApply "He₂"|].
+    iIntros "%w [Hτ HΓ₂] !>". 
     iApply (ewp_bind [ReplaceLCtx _]); first done. simpl.
-    iApply ewp_ms_prot_mono; [iApply sig_le_nil|].
     iApply (ewp_mono with "[HΓ₂]"); [by iApply "He₁"|].
     iIntros "%u [(%l & -> & Hinv) HΓ₃] !>".
     iApply (ewp_atomic _ (⊤ ∖ ↑tyN.@l)).
@@ -958,162 +847,36 @@ Section compatibility.
   
   (* Effect handling rules *)
   
-  Lemma sem_typed_perform_os Γ₁ Γ₂ e τ ρ' (A B : sem_sig Σ → sem_ty Σ → sem_ty Σ) 
+  Lemma sem_typed_perform Γ₁ Γ₂ e τ (A B : sem_sig Σ → sem_ty Σ → sem_ty Σ) 
     `{ NonExpansive2 A, NonExpansive2 B } :
-    let ρ := (μ∀TS: θ, α, A θ α ⇒ B θ α)%R in
-    Γ₁ ⊨ e : ⟨ρ, ρ'⟩ : A ρ τ ⊨ Γ₂ -∗
-    Γ₁ ⊨ (perform: e) : ⟨ρ, ρ'⟩ : B ρ τ ⊨ Γ₂.
+    let σ := (μ∀TS: θ, α, A θ α ⇒ B θ α)%S in
+    Γ₁ ⊨ e : σ : A σ τ ⊨ Γ₂ -∗
+    Γ₁ ⊨ (perform: e) : σ : B σ τ ⊨ Γ₂.
   Proof.
-    iIntros (ρ) "#He !# %vs HΓ₁ //=". rewrite /rec_perform.
-    iApply (ewp_bind [AppRCtx _; DoCtx OS; InjLCtx]); first done.
-    iApply (ewp_pers_mono with "[HΓ₁]"); [by iApply "He"|].
-    iIntros "!# %v [Hι HΓ₂] //= !>". ewp_pure_steps.
+    iIntros (σ) "#He !# %vs HΓ₁ //=". rewrite /rec_perform.
+    iApply (ewp_bind [AppRCtx _; DoCtx OS]); first done.
+    iApply (ewp_mono with "[HΓ₁]"); [by iApply "He"|].
+    iIntros "%v [Hι HΓ₂] //= !>". ewp_pure_steps.
     iApply ewp_do_os. rewrite upcl_sem_sig_rec_eff /=.
     iExists τ, v. iFrame. iSplitR; first done.
-    iIntros (b) "Hκ". ewp_pure_steps. iFrame.
+    iIntros "%b Hκ". ewp_pure_steps. iFrame "∗#".
   Qed.
 
-  Lemma sem_typed_perform_ms Γ₁ Γ₂ e τ ρ (A B : sem_sig Σ → sem_ty Σ → sem_ty Σ) 
-    `{ NonExpansive2 A, NonExpansive2 B } :
-    let ρ' := (μ∀TSₘ: θ, α, A θ α ⇒ B θ α)%R in
-    copy_env Γ₂ -∗
-    Γ₁ ⊨ e : ⟨ρ, ρ'⟩ : A ρ' τ ⊨ Γ₂ -∗
-    Γ₁ ⊨ (performₘ: e) : ⟨ρ, ρ'⟩ : B ρ' τ ⊨ Γ₂.
-  Proof.
-    iIntros (ρ') "#Hcpy #He !# %vs HΓ₁ //=". rewrite /rec_perform.
-    iApply (ewp_bind [AppRCtx _; DoCtx MS; InjRCtx]); first done.
-    iApply (ewp_pers_mono with "[HΓ₁]"); [by iApply "He"|].
-    iIntros "!# %v [Hι HΓ₂] //= !>". ewp_pure_steps.
-    iApply ewp_do_ms. rewrite upcl_sem_sig_rec_eff /=.
-    iExists τ, v. iFrame. iSplitR; first done.
-    iDestruct ("Hcpy" with "HΓ₂") as "#HΓ₂'".
-    iIntros "!# %b Hκ". ewp_pure_steps. iFrame "∗#".
-  Qed.
-
-  Lemma sem_typed_shallow_try Γ₁ Γ₂ Γ₃ Γ' x k e hos hms r A₁ B₁ A₂ B₂ τ τ' ρs 
-        `{NonExpansive2 A₁, NonExpansive2 B₁, NonExpansive2 A₂, NonExpansive2 B₂}:
-    x ∉ env_dom Γ₂ → x ∉ env_dom Γ' → k ∉ env_dom Γ' →
-    x ∉ env_dom Γ₃ → k ∉ env_dom Γ₃ → x ≠ k →
-    let ρ₁ := (μ∀TS: θ, α, A₁ θ α ⇒ B₁ θ α)%R in
-    let ρ₂ := (μ∀TSₘ: θ, α, A₂ θ α ⇒ B₂ θ α)%R in
-    Γ₁ ⊨ e : ⟨ρ₁, ρ₂⟩ : τ' ⊨ Γ₂ -∗
-    (∀ α, (x, A₁ ρ₁ α) :: (k, B₁ ρ₁ α -{ ⟨ρ₁, ρ₂⟩ }-∘ τ') :: Γ' ⊨ hos : ρs : τ ⊨ Γ₃) -∗
-    (∀ α, (x, A₂ ρ₂ α) :: (k, B₂ ρ₂ α -{ ⟨ρ₁, ρ₂⟩ }-> τ') :: Γ' ⊨ hms : ρs : τ ⊨ Γ₃) -∗
-    (x, τ') :: Γ₂ ++ Γ' ⊨ r : ρs : τ ⊨ Γ₃ -∗
-    Γ₁ ++ Γ' ⊨ (shallow-try-dual: e with
-                  effect  (λ: x k, hos) 
-                | effectₘ (λ: x k, hms) 
-                | return  (λ: x, r) end) : ρs : τ ⊨ Γ₃.
-  Proof.
-    iIntros (??????) "%ρ₁ %ρ₂ #He #Hhos #Hhms #Hr !# %vs HΓ₁Γ' //=".
-    iDestruct (env_sem_typed_app with "HΓ₁Γ'") as "[HΓ₁ HΓ']".
-    iApply (ewp_try_with _ _ _ (λ v, τ' v ∗ ⟦ Γ₂ ⟧ vs)%I with "[HΓ₁] [HΓ']"). 
-    { iApply (ewp_pers_mono with "[HΓ₁]"); [by iApply "He"|eauto]. }
-    iSplit; [|iSplit; iIntros (v c)].
-    - iIntros (v) "[Hv HΓ₂] //=". ewp_pure_steps.
-      rewrite -subst_map_insert.
-      iApply (ewp_pers_mono with "[HΓ₂ HΓ' Hv]"); [iApply "Hr"|].
-      { iExists v. rewrite env_sem_typed_app; solve_env. }
-      iIntros "!# % [Hτ HΓ₃]"; solve_env.
-    - rewrite upcl_sem_sig_rec_eff.
-      iIntros "(%α & %a & <- & Ha & Hκb) //=". rewrite /select_on_sum. ewp_pure_steps.
-      rewrite decide_True; [|split; first done; by injection].
-      rewrite subst_subst_ne; last done.
-      rewrite -subst_map_insert -delete_insert_ne; last done.
-      rewrite -subst_map_insert.
-      iApply (ewp_pers_mono with "[HΓ' Hκb Ha]"); [iApply "Hhos"; solve_env; iSplitR "HΓ'"|].
-      + iIntros (b) "Hκ /=".
-        iApply (ewp_pers_mono with "[Hκ Hκb]"); [by iApply "Hκb"|].
-        iIntros "!# % [Hτ' _] !> //=".
-      + by (do 2 (rewrite -env_sem_typed_insert; try done)).
-      + iIntros "!# %u [$ HΓ₃] !>".
-        rewrite -(env_sem_typed_insert _ _ x a); last done.
-        by rewrite -(env_sem_typed_insert _ _ k c).
-    - rewrite upcl_sem_sig_rec_eff.
-      iIntros "(%α & %a & <- & Ha & Hκb) //=". rewrite /select_on_sum. ewp_pure_steps.
-      rewrite decide_True; [|split; first done; by injection].
-      rewrite subst_subst_ne; last done.
-      rewrite -subst_map_insert -delete_insert_ne; last done.
-      rewrite -subst_map_insert.
-      iApply (ewp_pers_mono with "[HΓ' Hκb Ha]"); [iApply "Hhms"; solve_env|].
-      + iDestruct "Hκb" as "#Hκb".
-        iIntros "!# %b Hκ /=".
-        iApply (ewp_pers_mono with "[Hκ]"); [by iApply "Hκb"|].
-        iIntros "!# % [Hτ' _] !> //=".
-      + by (do 2 (rewrite -env_sem_typed_insert; try done)).
-      + iIntros "!# %u [$ HΓ₃] !>".
-        rewrite -(env_sem_typed_insert _ _ x a); last done.
-        by rewrite -(env_sem_typed_insert _ _ k c).
-  Qed.
-  
-  Lemma sem_typed_shallow_try_os Γ₁ Γ₂ Γ' x k e h r A₁ B₁ A₂ B₂ τ τ' ρ₁' 
-        `{NonExpansive2 A₁, NonExpansive2 B₁, NonExpansive2 A₂, NonExpansive2 B₂}:
-    x ∉ env_dom Γ₂ → x ∉ env_dom Γ' → k ∉ env_dom Γ' → x ≠ k → 
-    let ρ₁ := (μ∀TS: θ, α, A₁ θ α ⇒ B₁ θ α)%R in
-    let ρ₂ := (μ∀TSₘ: θ, α, A₂ θ α ⇒ B₂ θ α)%R in
-    let ρs := ⟨ ρ₁', ρ₂ ⟩%R in
-    copy_env Γ' -∗
-    Γ₁ ⊨ e : ⟨ρ₁, ρ₂⟩ : τ' ⊨ Γ₂ -∗
-    (∀ α, (x, A₁ ρ₁ α) :: (k, B₁ ρ₁ α -{ ⟨ρ₁, ρ₂⟩ }-∘ τ') :: Γ' ⊨ h : ρs : τ ⊨ Γ') -∗
-    (x, τ') :: Γ₂ ++ Γ' ⊨ r : ρs : τ ⊨ Γ' -∗
-    Γ₁ ++ Γ' ⊨ (shallow-try-os: e with
-                  effect  (λ: x k, h)
-                | return  (λ: x, r) end) : ρs : τ ⊨ Γ'.
-  Proof.
-    iIntros (????) "%ρ₁ %ρ₂ %ρs #Hcpy #He #Hh #Hr !# %vs HΓ₁Γ'".
-    iDestruct (env_sem_typed_app with "HΓ₁Γ'") as "[HΓ₁ HΓ']". simpl. 
-    do 12 ewp_value_or_step.
-    iSpecialize ("He" with "HΓ₁"). iRevert "He".
-    iLöb as "IH" forall (e). iIntros "He". ewp_pure_steps.
-    iApply (ewp_try_with _ _ _ (λ v, τ' v ∗ ⟦ Γ₂ ⟧ vs)%I with "[He] [HΓ']"). 
-    { ewp_pure_steps. by iApply "He". }
-    iSplit; [|iSplit; iIntros (v c)].
-    - iIntros (v) "[Hv HΓ₂] //=". ewp_pure_steps.
-      rewrite -subst_map_insert. 
-      iApply (ewp_pers_mono with "[HΓ₂ HΓ' Hv]"); [iApply "Hr"|].
-      { rewrite app_comm_cons env_sem_typed_app. iSplitR "HΓ'"; solve_env. }
-      iIntros "!# % [$ HΓ₃] !>". solve_env.
-    - rewrite upcl_sem_sig_rec_eff.
-      iIntros "(%α & %a & <- & Ha & Hκb) //=". rewrite /select_on_sum. ewp_pure_steps.
-      solve_dec.
-      rewrite subst_subst_ne; last done. rewrite -subst_map_insert. 
-      rewrite -delete_insert_ne; last done. rewrite -subst_map_insert.
-      iApply (ewp_pers_mono with "[HΓ' Hκb Ha]"); [iApply "Hh"; solve_env; iSplitL "Hκb"|].
-      + iIntros "%b Hκ /=".
-        iApply (ewp_pers_mono with "[Hκ Hκb]"); [by iApply "Hκb"|].
-        iIntros "!# % [Hτ' _] !> //=".
-      + by (do 2 (rewrite -env_sem_typed_insert; try done)).
-      + iIntros "!# %u [$ HΓ₃] !>".
-        by do 2 (rewrite -env_sem_typed_insert; last done).
-    - rewrite upcl_sem_sig_rec_eff.
-      iIntros "(%α & %a & <- & Ha & Hκb) //=". rewrite /select_on_sum. ewp_pure_steps.
-      iDestruct "Hκb" as "#Hκb". iApply ewp_do_ms. 
-      rewrite upcl_sem_sig_rec_eff. simpl. iExists _, a. iSplitR; first done.
-      iSplitL "Ha"; first iFrame. 
-      iDestruct ("Hcpy" with "HΓ'") as "#HΓ''".
-      iIntros "!# %b HB₁". rewrite /rec_perform. do 7 ewp_value_or_step.
-      iSpecialize ("IH" $! (c b)%E with "HΓ''"). 
-      iApply "IH". simpl. by iApply "Hκb".
-  Qed.
-
-  Lemma sem_typed_shallow_try_os' Γ₁ Γ₂ Γ₃ Γ' x k e h r A₁ B₁ τ τ' ρ₁' 
-        `{NonExpansive2 A₁, NonExpansive2 B₁ }:
+  Lemma sem_typed_shallow_try Γ₁ Γ₂ Γ₃ Γ' x k e h r A B τ τ' σ' `{NonExpansive2 A, NonExpansive2 B }:
     x ∉ env_dom Γ₂ → x ∉ env_dom Γ' → x ∉ env_dom Γ₃ → k ∉ env_dom Γ₃ → k ∉ env_dom Γ' → x ≠ k →
-    let ρ₁ := (μ∀TS: θ, α, A₁ θ α ⇒ B₁ θ α)%R in
-    let ρs := ⟨ ρ₁', ⟩%R in
-    Γ₁ ⊨ e : ⟨ρ₁, ⟩ : τ' ⊨ Γ₂ -∗
-    (∀ α, (x, A₁ ρ₁ α) :: (k, B₁ ρ₁ α -{ ⟨ρ₁, ⟩ }-∘ τ') :: Γ' ⊨ h : ρs : τ ⊨ Γ₃) -∗
-    (x, τ') :: Γ₂ ++ Γ' ⊨ r : ρs : τ ⊨ Γ₃ -∗
-    Γ₁ ++ Γ' ⊨ (shallow-try-os: e with
+    let σ := (μ∀TS: θ, α, A θ α ⇒ B θ α)%S in
+    Γ₁ ⊨ e : σ : τ ⊨ Γ₂ -∗
+    (∀ α, (x, A σ α) :: (k, B σ α -{ σ }-∘ τ) :: Γ' ⊨ h : σ' : τ' ⊨ Γ₃) -∗
+    (x, τ) :: Γ₂ ++ Γ' ⊨ r : σ' : τ' ⊨ Γ₃ -∗
+    Γ₁ ++ Γ' ⊨ (shallow-try: e with
                   effect  (λ: x k, h)
-                | return  (λ: x, r) end) : ρs : τ ⊨ Γ₃.
+                | return  (λ: x, r) end) : σ' : τ' ⊨ Γ₃.
   Proof.
-    iIntros (??????) "%ρ₁ %ρs #He #Hh #Hr !# %vs HΓ₁Γ'".
+    iIntros (??????) "%σ #He #Hh #Hr !# %vs HΓ₁Γ'".
     iDestruct (env_sem_typed_app with "HΓ₁Γ'") as "[HΓ₁ HΓ']". simpl. 
-    do 12 ewp_value_or_step.
     iSpecialize ("He" with "HΓ₁"). iRevert "He".
-    iLöb as "IH" forall (e). iIntros "He". ewp_pure_steps.
-    iApply (ewp_try_with _ _ _ (λ v, τ' v ∗ ⟦ Γ₂ ⟧ vs)%I with "[He] [HΓ']"). 
+    iLöb as "IH" forall (e). iIntros "He".
+    iApply (ewp_try_with _ _ _ (λ v, τ v ∗ ⟦ Γ₂ ⟧ vs)%I with "[He] [HΓ']"). 
     { ewp_pure_steps. by iApply "He". }
     iSplit; [|iSplit; iIntros (v c)].
     - iIntros (v) "[Hv HΓ₂] //=". ewp_pure_steps.
@@ -1122,148 +885,36 @@ Section compatibility.
       { rewrite app_comm_cons env_sem_typed_app. iSplitR "HΓ'"; solve_env. }
       iIntros "!# % [$ HΓ₃] !>". solve_env.
     - rewrite upcl_sem_sig_rec_eff.
-      iIntros "(%α & %a & <- & Ha & Hκb) //=". rewrite /select_on_sum. ewp_pure_steps.
+      iIntros "(%α & %a & <- & Ha & Hκb) //=". ewp_pure_steps.
       solve_dec.
       rewrite subst_subst_ne; last done. rewrite -subst_map_insert. 
       rewrite -delete_insert_ne; last done. rewrite -subst_map_insert.
-      iApply (ewp_pers_mono with "[HΓ' Hκb Ha]"); [iApply "Hh"; solve_env; iSplitL "Hκb"|].
+      iApply (ewp_mono with "[HΓ' Hκb Ha]"); [iApply "Hh"; solve_env; iSplitL "Hκb"|].
       + iIntros "%b Hκ /=".
-        iApply (ewp_pers_mono with "[Hκ Hκb]"); [by iApply "Hκb"|].
-        iIntros "!# % [Hτ' _] !> //=".
+        iApply (ewp_mono with "[Hκ Hκb]"); [by iApply "Hκb"|].
+        iIntros "% [Hτ' _] !> //=".
       + by (do 2 (rewrite -env_sem_typed_insert; try done)).
-      + iIntros "!# %u [$ HΓ₃] !>".
+      + iIntros "%u [$ HΓ₃] !>".
         by do 2 (rewrite -env_sem_typed_insert; last done).
     - iIntros "/= (% & [] & ?)".
   Qed.
 
-  Lemma sem_typed_shallow_try_ms Γ₁ Γ₂ Γ' x k e h r A₁ B₁ A₂ B₂ τ τ' ρ₂' 
-        `{NonExpansive2 A₁, NonExpansive2 B₁, NonExpansive2 A₂, NonExpansive2 B₂}:
-    x ∉ env_dom Γ₂ → x ∉ env_dom Γ' → k ∉ env_dom Γ' → x ≠ k → 
-    let ρ₁ := (μ∀TS: θ, α, A₁ θ α ⇒ B₁ θ α)%R in
-    let ρ₂ := (μ∀TSₘ: θ, α, A₂ θ α ⇒ B₂ θ α)%R in
-    let ρs := ⟨ ρ₁, ρ₂' ⟩%R in
-    Γ₁ ⊨ e : ⟨ρ₁, ρ₂⟩ : τ' ⊨ Γ₂ -∗
-    (∀ α, (x, A₂ ρ₂ α) :: (k, B₂ ρ₂ α -{ ⟨ρ₁, ρ₂⟩ }-> τ') :: Γ' ⊨ h : ρs : τ ⊨ Γ') -∗
-    (x, τ') :: Γ₂ ++ Γ' ⊨ r : ρs : τ ⊨ Γ' -∗
-    Γ₁ ++ Γ' ⊨ (shallow-try-ms: e with
-                  effectₘ (λ: x k, h)
-                | return  (λ: x, r) end) : ρs : τ ⊨ Γ'.
-  Proof.
-    iIntros (????) "%ρ₁ %ρ₂ %ρs #He #Hh #Hr !# %vs HΓ₁Γ'".
-    iDestruct (env_sem_typed_app with "HΓ₁Γ'") as "[HΓ₁ HΓ']". simpl.
-    do 12 ewp_value_or_step.
-    iSpecialize ("He" with "HΓ₁"). iRevert "He".
-    iLöb as "IH" forall (e). iIntros "He". ewp_pure_steps.
-    iApply (ewp_try_with _ _ _ (λ v, τ' v ∗ ⟦ Γ₂ ⟧ vs)%I with "[He] [HΓ']"). 
-    { ewp_pure_steps. by iApply "He". }
-    iSplit; [|iSplit; iIntros (v c)].
-    - iIntros (v) "[Hv HΓ₂] //=". ewp_pure_steps.
-      rewrite -subst_map_insert.
-      iApply (ewp_pers_mono with "[HΓ₂ HΓ' Hv]"); [iApply "Hr"|].
-      { rewrite app_comm_cons env_sem_typed_app. iSplitR "HΓ'"; solve_env. }
-      iIntros "!# % [$ HΓ₃] !>". solve_env.
-    - rewrite upcl_sem_sig_rec_eff.
-      iIntros "(%α & %a & <- & Ha & Hκb) //=". rewrite /select_on_sum. ewp_pure_steps.
-      iApply ewp_do_os. 
-      rewrite upcl_sem_sig_rec_eff. simpl. iExists _, a. iSplitR; first done.
-      iSplitL "Ha"; first iFrame. 
-      iIntros "%b HB₁". rewrite /rec_perform. do 7 ewp_value_or_step.
-      iSpecialize ("IH" $! (c b)%E with "HΓ'"). 
-      iApply "IH". simpl. by iApply "Hκb".
-    - rewrite upcl_sem_sig_rec_eff.
-      iIntros "(%α & %a & <- & Ha & Hκb) //=". rewrite /select_on_sum. ewp_pure_steps.
-      solve_dec.
-      rewrite subst_subst_ne; last done. rewrite -subst_map_insert. 
-      rewrite -delete_insert_ne; last done. rewrite -subst_map_insert.
-      iApply (ewp_pers_mono with "[HΓ' Hκb Ha]"); [iApply "Hh"; solve_env|].
-      + iDestruct "Hκb" as "#Hκb".
-        iIntros "!# %b Hκ /=".
-        iApply (ewp_pers_mono with "[Hκ Hκb]"); [by iApply "Hκb"|].
-        iIntros "!# % [Hτ' _] !> //=".
-      + by (do 2 (rewrite -env_sem_typed_insert; try done)).
-      + iIntros "!# %u [$ HΓ₃] !>".
-        by do 2 (rewrite -env_sem_typed_insert; last done).
-  Qed.
-
-  Lemma sem_typed_deep_try Γ₁ Γ₂ Γ₃ Γ' x k e hos hms r A₁ B₁ A₂ B₂ τ τ' ρs 
-        `{NonExpansive2 A₁, NonExpansive2 B₁, NonExpansive2 A₂, NonExpansive2 B₂}:
+  Lemma sem_typed_deep_try Γ₁ Γ₂ Γ' Γ₃ x k e h r A B τ τ' σ' `{NonExpansive2 A, NonExpansive2 B}:
     x ∉ env_dom Γ₂ → x ∉ env_dom Γ' → k ∉ env_dom Γ' →
     x ∉ env_dom Γ₃ → k ∉ env_dom Γ₃ → x ≠ k → 
-    let ρ₁ := (μ∀TS: θ, α, A₁ θ α ⇒ B₁ θ α)%R in
-    let ρ₂ := (μ∀TSₘ: θ, α, A₂ θ α ⇒ B₂ θ α)%R in
+    let σ := (μ∀TS: θ, α, A θ α ⇒ B θ α)%S in
     copy_env Γ' -∗
-    Γ₁ ⊨ e : ⟨ρ₁, ρ₂⟩ : τ' ⊨ Γ₂ -∗
-    (∀ α, (x, A₁ ρ₁ α) :: (k, B₁ ρ₁ α -{ ρs }-∘ τ) :: Γ' ⊨ hos : ρs : τ ⊨ Γ₃) -∗
-    (∀ α, (x, A₂ ρ₂ α) :: (k, B₂ ρ₂ α -{ ρs }-> τ) :: Γ' ⊨ hms : ρs : τ ⊨ Γ₃) -∗
-    (x, τ') :: Γ₂ ++ Γ' ⊨ r : ρs : τ ⊨ Γ₃ -∗
-    Γ₁ ++ Γ' ⊨ (deep-try-dual: e with
-                  effect  (λ: x k, hos) 
-                | effectₘ (λ: x k, hms) 
-                | return  (λ: x, r) end) : ρs : τ ⊨ Γ₃.
-  Proof.
-    iIntros (??????) "%ρ₁ %ρ₂ #Hcpy #He #Hhos #Hhms #Hr !# %vs HΓ₁Γ' //=".
-    iDestruct (env_sem_typed_app with "HΓ₁Γ'") as "[HΓ₁ HΓ'']".
-    iDestruct ("Hcpy" with "HΓ''") as "#HΓ'".
-    rewrite /select_on_sum. ewp_pure_steps. 
-    iApply (ewp_deep_try_with _ _ _ (λ v, τ' v ∗ env_sem_typed Γ₂ vs) with "[HΓ₁] []").
-    { iApply (ewp_pers_mono with "[HΓ₁]"); [by iApply "He"|eauto]. }
-    iLöb as "IH". rewrite {2}deep_handler_unfold.
-    iSplit; [|iSplit; iIntros (v c)].
-    - iIntros (v) "[Hv HΓ₂] //=". ewp_pure_steps.
-      rewrite -subst_map_insert.
-      iApply (ewp_pers_mono with "[HΓ₂ HΓ' Hv]"); [iApply "Hr"|].
-      { iExists v. rewrite env_sem_typed_app; solve_env. }
-      iIntros "!# % [Hτ HΓ₃]"; solve_env.
-    - rewrite upcl_sem_sig_rec_eff.
-      iIntros "(%α & %a & <- & Ha & Hκb) //=". ewp_pure_steps.
-      rewrite decide_True; [|split; first done; by injection].
-      rewrite subst_subst_ne; last done.
-      rewrite -subst_map_insert -delete_insert_ne; last done.
-      rewrite -subst_map_insert.
-      iApply (ewp_pers_mono with "[HΓ' Hκb Ha]"); [iApply "Hhos"; solve_env; iSplitR "HΓ'"|].
-      + iIntros (b) "Hκ /=".
-        iApply (ewp_pers_mono with "[Hκ Hκb]"); [iApply ("Hκb" with "Hκ IH")|].
-        iIntros "!# % [Hτ' _] !> //=".
-      + by (do 2 (rewrite -env_sem_typed_insert; try done)).
-      + iIntros "!# %u [$ HΓ₃] !>".
-        rewrite -(env_sem_typed_insert _ _ x a); last done.
-        by rewrite -(env_sem_typed_insert _ _ k c).
-    - rewrite upcl_sem_sig_rec_eff.
-      iIntros "(%α & %a & <- & Ha & Hκb) //=". ewp_pure_steps.
-      rewrite decide_True; [|split; first done; by injection].
-      rewrite subst_subst_ne; last done.
-      rewrite -subst_map_insert -delete_insert_ne; last done.
-      rewrite -subst_map_insert.
-      iApply (ewp_pers_mono with "[HΓ' Hκb Ha]"); [iApply "Hhms"; solve_env|].
-      + iDestruct "Hκb" as "#Hκb".
-        iIntros "!# %b Hκ /=".
-        iApply (ewp_pers_mono with "[Hκ]"); [iApply ("Hκb" with "Hκ IH")|].
-        iIntros "!# % [Hτ' _] !> //=".
-      + by (do 2 (rewrite -env_sem_typed_insert; try done)).
-      + iIntros "!# %u [$ HΓ₃] !>".
-        rewrite -(env_sem_typed_insert _ _ x a); last done.
-        by rewrite -(env_sem_typed_insert _ _ k c).
-  Qed.
-
-  Lemma sem_typed_deep_try_os Γ₁ Γ₂ Γ' x k e h r A₁ B₁ A₂ B₂ τ τ' ρ₁' 
-        `{NonExpansive2 A₁, NonExpansive2 B₁, NonExpansive2 A₂, NonExpansive2 B₂}:
-    x ∉ env_dom Γ₂ → x ∉ env_dom Γ' → k ∉ env_dom Γ' → x ≠ k → 
-    let ρ₁ := (μ∀TS: θ, α, A₁ θ α ⇒ B₁ θ α)%R in
-    let ρ₂ := (μ∀TSₘ: θ, α, A₂ θ α ⇒ B₂ θ α)%R in
-    let ρs := ⟨ρ₁', ρ₂⟩%R in
-    copy_env Γ' -∗
-    Γ₁ ⊨ e : ⟨ρ₁, ρ₂⟩ : τ' ⊨ Γ₂ -∗
-    (∀ α, (x, A₁ ρ₁ α) :: (k, B₁ ρ₁ α -{ ρs }-∘ τ) :: Γ' ⊨ h : ρs : τ ⊨ Γ') -∗
-    (x, τ') :: Γ₂ ++ Γ' ⊨ r : ρs : τ ⊨ Γ' -∗
-    Γ₁ ++ Γ' ⊨ (deep-try-os: e with
+    Γ₁ ⊨ e : σ : τ ⊨ Γ₂ -∗
+    (∀ α, (x, A σ α) :: (k, B σ α -{ σ' }-∘ τ') :: Γ' ⊨ h : σ' : τ' ⊨ Γ₃) -∗
+    (x, τ) :: Γ₂ ++ Γ' ⊨ r : σ' : τ' ⊨ Γ₃ -∗
+    Γ₁ ++ Γ' ⊨ (deep-try: e with
                   effect  (λ: x k, h) 
-                | return  (λ: x, r) end) : ρs : τ ⊨ Γ'.
+                | return  (λ: x, r) end) : σ' : τ' ⊨ Γ₃.
   Proof.
-    iIntros (????) "%ρ₁ %ρ₂ %ρs #Hcpy #He #Hh #Hr !# %vs HΓ₁Γ' //=".
+    iIntros (??????) "%σ #Hcpy #He #Hh #Hr !# %vs HΓ₁Γ' //=".
     iDestruct (env_sem_typed_app with "HΓ₁Γ'") as "[HΓ₁ HΓ'']".
-    iDestruct ("Hcpy" with "HΓ''") as "#HΓ'".
-    rewrite /select_on_sum. ewp_pure_steps. 
-    iApply (ewp_deep_try_with _ _ _ (λ v, τ' v ∗ env_sem_typed Γ₂ vs) with "[HΓ₁] []").
+    iDestruct ("Hcpy" with "HΓ''") as "#HΓ'". ewp_pure_steps. 
+    iApply (ewp_deep_try_with _ _ _ (λ v, τ v ∗ env_sem_typed Γ₂ vs) with "[HΓ₁] []").
     { by iApply "He". }
     iLöb as "IH". rewrite {2}deep_handler_unfold.
     iSplit; [|iSplit; iIntros (v c)].
@@ -1278,116 +929,15 @@ Section compatibility.
       rewrite subst_subst_ne; last done.
       rewrite -subst_map_insert -delete_insert_ne; last done.
       rewrite -subst_map_insert.
-      iApply (ewp_pers_mono with "[HΓ' Hκb Ha]"); [iApply "Hh"; solve_env; iSplitR "HΓ'"|].
+      iApply (ewp_mono with "[HΓ' Hκb Ha]"); [iApply "Hh"; solve_env; iSplitR "HΓ'"|].
       + iIntros (b) "Hκ /=".
-        iApply (ewp_pers_mono with "[Hκ Hκb]"); [iApply ("Hκb" with "Hκ IH")|].
-        iIntros "!# % [Hτ' _] !> //=".
+        iApply (ewp_mono with "[Hκ Hκb]"); [iApply ("Hκb" with "Hκ IH")|].
+        iIntros "% [Hτ' _] !> //=".
       + by (do 2 (rewrite -env_sem_typed_insert; try done)).
-      + iIntros "!# %u [$ HΓ₃] !>".
-        rewrite -(env_sem_typed_insert _ _ x a); last done.
-        by rewrite -(env_sem_typed_insert _ _ k c).
-    - rewrite upcl_sem_sig_rec_eff.
-      iIntros "(%α & %a & <- & Ha & Hκb) //=". ewp_pure_steps.
-      iApply ewp_do_ms.
-      rewrite upcl_sem_sig_rec_eff. simpl. iExists _, a. iSplitR; first done.
-      iSplitL "Ha"; first iFrame. iDestruct "Hκb" as "#Hκb".
-      iIntros "!# %b HB₁". rewrite /rec_perform. ewp_pure_steps.
-      iApply ("Hκb" with "HB₁"). iApply "IH".
-  Qed.
-    
-  Lemma sem_typed_deep_try_os' Γ₁ Γ₂ Γ' Γ₃ x k e h r A₁ B₁ τ τ' ρ₁' 
-        `{NonExpansive2 A₁, NonExpansive2 B₁}:
-    x ∉ env_dom Γ₂ → x ∉ env_dom Γ' → k ∉ env_dom Γ' →
-    x ∉ env_dom Γ₃ → k ∉ env_dom Γ₃ → x ≠ k → 
-    let ρ₁ := (μ∀TS: θ, α, A₁ θ α ⇒ B₁ θ α)%R in
-    let ρs := ⟨ρ₁',⟩%R in
-    copy_env Γ' -∗
-    Γ₁ ⊨ e : ⟨ρ₁,⟩ : τ' ⊨ Γ₂ -∗
-    (∀ α, (x, A₁ ρ₁ α) :: (k, B₁ ρ₁ α -{ ρs }-∘ τ) :: Γ' ⊨ h : ρs : τ ⊨ Γ₃) -∗
-    (x, τ') :: Γ₂ ++ Γ' ⊨ r : ρs : τ ⊨ Γ₃ -∗
-    Γ₁ ++ Γ' ⊨ (deep-try-os: e with
-                  effect  (λ: x k, h) 
-                | return  (λ: x, r) end) : ρs : τ ⊨ Γ₃.
-  Proof.
-    iIntros (??????) "%ρ₁ %ρs #Hcpy #He #Hh #Hr !# %vs HΓ₁Γ' //=".
-    iDestruct (env_sem_typed_app with "HΓ₁Γ'") as "[HΓ₁ HΓ'']".
-    iDestruct ("Hcpy" with "HΓ''") as "#HΓ'".
-    rewrite /select_on_sum. ewp_pure_steps. 
-    iApply (ewp_deep_try_with _ _ _ (λ v, τ' v ∗ env_sem_typed Γ₂ vs) with "[HΓ₁] []").
-    { by iApply "He". }
-    iLöb as "IH". rewrite {2}deep_handler_unfold.
-    iSplit; [|iSplit; iIntros (v c)].
-    - iIntros (v) "[Hv HΓ₂] //=". ewp_pure_steps.
-      rewrite -subst_map_insert.
-      iApply (ewp_pers_mono with "[HΓ₂ HΓ' Hv]"); [iApply "Hr"|].
-      { iExists v. rewrite env_sem_typed_app; solve_env. }
-      iIntros "!# % [Hτ HΓ₃]"; solve_env.
-    - rewrite upcl_sem_sig_rec_eff.
-      iIntros "(%α & %a & <- & Ha & Hκb) //=". ewp_pure_steps.
-      rewrite decide_True; [|split; first done; by injection].
-      rewrite subst_subst_ne; last done.
-      rewrite -subst_map_insert -delete_insert_ne; last done.
-      rewrite -subst_map_insert.
-      iApply (ewp_pers_mono with "[HΓ' Hκb Ha]"); [iApply "Hh"; solve_env; iSplitR "HΓ'"|].
-      + iIntros (b) "Hκ /=".
-        iApply (ewp_pers_mono with "[Hκ Hκb]"); [iApply ("Hκb" with "Hκ IH")|].
-        iIntros "!# % [Hτ' _] !> //=".
-      + by (do 2 (rewrite -env_sem_typed_insert; try done)).
-      + iIntros "!# %u [$ HΓ₃] !>".
+      + iIntros "%u [$ HΓ₃] !>".
         rewrite -(env_sem_typed_insert _ _ x a); last done.
         by rewrite -(env_sem_typed_insert _ _ k c).
     - simpl. iIntros "(% & [] & ?)".
-  Qed.
-
-  Lemma sem_typed_deep_try_ms Γ₁ Γ₂ Γ' x k e h r A₁ B₁ A₂ B₂ τ τ' ρ₂' 
-        `{NonExpansive2 A₁, NonExpansive2 B₁, NonExpansive2 A₂, NonExpansive2 B₂}:
-    x ∉ env_dom Γ₂ → x ∉ env_dom Γ' → k ∉ env_dom Γ' → x ≠ k → 
-    let ρ₁ := (μ∀TS: θ, α, A₁ θ α ⇒ B₁ θ α)%R in
-    let ρ₂ := (μ∀TSₘ: θ, α, A₂ θ α ⇒ B₂ θ α)%R in
-    let ρs := ⟨ρ₁, ρ₂'⟩%R in
-    copy_env Γ' -∗
-    Γ₁ ⊨ e : ⟨ρ₁, ρ₂⟩ : τ' ⊨ Γ₂ -∗
-    (∀ α, (x, A₂ ρ₂ α) :: (k, B₂ ρ₂ α -{ ρs }-> τ) :: Γ' ⊨ h : ρs : τ ⊨ Γ') -∗
-    (x, τ') :: Γ₂ ++ Γ' ⊨ r : ρs : τ ⊨ Γ' -∗
-    Γ₁ ++ Γ' ⊨ (deep-try-ms: e with
-                  effectₘ (λ: x k, h) 
-                | return  (λ: x, r) end) : ρs : τ ⊨ Γ'.
-  Proof.
-    iIntros (????) "%ρ₁ %ρ₂ %ρs #Hcpy #He #Hh #Hr !# %vs HΓ₁Γ' //=".
-    iDestruct (env_sem_typed_app with "HΓ₁Γ'") as "[HΓ₁ HΓ'']".
-    iDestruct ("Hcpy" with "HΓ''") as "#HΓ'".
-    rewrite /select_on_sum. ewp_pure_steps. 
-    iApply (ewp_deep_try_with _ _ _ (λ v, τ' v ∗ env_sem_typed Γ₂ vs) with "[HΓ₁] []").
-    { by iApply "He". }
-    iLöb as "IH". rewrite {2}deep_handler_unfold.
-    iSplit; [|iSplit; iIntros (v c)].
-    - iIntros (v) "[Hv HΓ₂] //=". ewp_pure_steps.
-      rewrite -subst_map_insert.
-      iApply (ewp_pers_mono with "[HΓ₂ HΓ' Hv]"); [iApply "Hr"|].
-      { iExists v. rewrite env_sem_typed_app; solve_env. }
-      iIntros "!# % [Hτ HΓ₃]"; solve_env.
-    - rewrite upcl_sem_sig_rec_eff.
-      iIntros "(%α & %a & <- & Ha & Hκb) //=". ewp_pure_steps.
-      iApply ewp_do_os.
-      rewrite upcl_sem_sig_rec_eff. simpl. iExists _, a. iSplitR; first done.
-      iSplitL "Ha"; first iFrame. 
-      iIntros (b) "HB₁". rewrite /rec_perform. ewp_pure_steps.
-      iApply ("Hκb" with "HB₁"). iApply "IH".
-    - rewrite upcl_sem_sig_rec_eff.
-      iIntros "(%α & %a & <- & Ha & Hκb) //=". ewp_pure_steps.
-      rewrite decide_True; [|split; first done; by injection].
-      rewrite subst_subst_ne; last done.
-      rewrite -subst_map_insert -delete_insert_ne; last done.
-      rewrite -subst_map_insert.
-      iApply (ewp_pers_mono with "[HΓ' Hκb Ha]"); [iApply "Hh"; solve_env|].
-      + iDestruct "Hκb" as "#Hκb".
-        iIntros "!# %b Hκ /=".
-        iApply (ewp_pers_mono with "[Hκ Hκb]"); [iApply ("Hκb" with "Hκ IH")|].
-        iIntros "!# % [Hτ' _] !> //=".
-      + by (do 2 (rewrite -env_sem_typed_insert; try done)).
-      + iIntros "!# %u [$ HΓ₃] !>".
-        rewrite -(env_sem_typed_insert _ _ x a); last done.
-        by rewrite -(env_sem_typed_insert _ _ k c).
   Qed.
 
 End compatibility.
